wip: specialized bignum

code/k256/Hacl.Impl.K256.Point.fst
@@ -11,8 +11,9 @@ module ST = FStar.HyperStack.ST
 module LSeq = Lib.Sequence
 module BSeq = Lib.ByteSequence
 
-module SD = Hacl.Spec.Bignum.Definitions
 module S = Spec.K256
+module BI = Hacl.Spec.K256.Field52
+module BL = Hacl.Spec.K256.Field52.Lemmas
 
 open Hacl.K256.Field
 
@@ -22,62 +23,63 @@ open Hacl.K256.Field
 
 // (_X, _Y, _Z)
 inline_for_extraction noextract
-let point = lbuffer uint64 (nlimb *! 3ul)
+let point = lbuffer uint64 15ul
 
 inline_for_extraction noextract
 let getx (p:point) : Stack felem
   (requires fun h -> live h p)
-  (ensures fun h0 f h1 -> f == gsub p 0ul nlimb /\ h0 == h1)
-  = sub p 0ul nlimb
+  (ensures fun h0 f h1 -> f == gsub p 0ul 5ul /\ h0 == h1)
+  = sub p 0ul 5ul
 
 inline_for_extraction noextract
 let gety (p:point) : Stack felem
   (requires fun h -> live h p)
-  (ensures fun h0 f h1 -> f == gsub p nlimb nlimb /\ h0 == h1)
-  = sub p nlimb nlimb
+  (ensures fun h0 f h1 -> f == gsub p 5ul 5ul /\ h0 == h1)
+  = sub p 5ul 5ul
 
 inline_for_extraction noextract
 let getz (p:point) : Stack felem
   (requires fun h -> live h p)
-  (ensures fun h0 f h1 -> f == gsub p (2ul *! nlimb) nlimb /\ h0 == h1)
-  = sub p (2ul *! nlimb) nlimb
+  (ensures fun h0 f h1 -> f == gsub p 10ul 5ul /\ h0 == h1)
+  = sub p 10ul 5ul
 
 
-noextract
-let point_inv_lseq (p:LSeq.lseq uint64 12) =
-  SD.bn_v (LSeq.sub p 0 4) < S.prime /\
-  SD.bn_v (LSeq.sub p 4 4) < S.prime /\
-  SD.bn_v (LSeq.sub p 8 4) < S.prime
+inline_for_extraction noextract
+let as_felem5_lseq (s:LSeq.lseq uint64 5) : felem5 =
+  let open Lib.Sequence in
+  (s.[0],s.[1],s.[2],s.[3],s.[4])
 
-noextract
+
+inline_for_extraction noextract
+let point_inv_lseq (p:LSeq.lseq uint64 15) =
+  inv_lazy_reduced2_5 (as_felem5_lseq (LSeq.sub p 0 5)) /\
+  inv_lazy_reduced2_5 (as_felem5_lseq (LSeq.sub p 5 5)) /\
+  inv_lazy_reduced2_5 (as_felem5_lseq (LSeq.sub p 10 5))
+
+inline_for_extraction noextract
 let point_inv (h:mem) (p:point) =
-  point_inv_lseq (as_seq h p)
+  inv_lazy_reduced2 h (gsub p 0ul 5ul) /\
+  inv_lazy_reduced2 h (gsub p 5ul 5ul) /\
+  inv_lazy_reduced2 h (gsub p 10ul 5ul)
 
-noextract
-let point_as_nat3_lseq (p:LSeq.lseq uint64 12) =
-  (SD.bn_v (LSeq.sub p 0 4),
-   SD.bn_v (LSeq.sub p 4 4),
-   SD.bn_v (LSeq.sub p 8 4))
+inline_for_extraction noextract
+let point_nat (h:mem) (p:point) =
+ (as_nat h (gsub p 0ul 5ul),
+  as_nat h (gsub p 5ul 5ul),
+  as_nat h (gsub p 10ul 5ul))
 
-noextract
-let point_as_nat3 (h:mem) (p:point) =
-  point_as_nat3_lseq (as_seq h p)
 
-noextract
-let point_as_nat3_proj_lseq (p:LSeq.lseq uint64 12{point_inv_lseq p}) : GTot S.proj_point =
-  (SD.bn_v (LSeq.sub p 0 4),
-   SD.bn_v (LSeq.sub p 4 4),
-   SD.bn_v (LSeq.sub p 8 4))
+inline_for_extraction noextract
+let point_eval_lseq (p:LSeq.lseq uint64 15) : GTot S.proj_point =
+ (feval5 (as_felem5_lseq (LSeq.sub p 0 5)),
+  feval5 (as_felem5_lseq (LSeq.sub p 5 5)),
+  feval5 (as_felem5_lseq (LSeq.sub p 10 5)))
 
-noextract
-let point_as_nat3_proj (h:mem) (p:point{point_inv h p}) : GTot S.proj_point =
-  point_as_nat3_proj_lseq (as_seq h p)
-
-noextract
-let point_eval (h:mem) (p:point) =
-  (feval h (gsub p 0ul nlimb),
-   feval h (gsub p nlimb nlimb),
-   feval h (gsub p (2ul *! nlimb) nlimb))
+inline_for_extraction noextract
+let point_eval (h:mem) (p:point) : GTot S.proj_point =
+ (feval h (gsub p 0ul 5ul),
+  feval h (gsub p 5ul 5ul),
+  feval h (gsub p 10ul 5ul))
 
 
 ///  Create a point
@@ -86,28 +88,21 @@ inline_for_extraction noextract
 val create_point: unit -> StackInline point
   (requires fun h -> True)
   (ensures  fun h0 f h1 ->
-    stack_allocated f h0 h1 (LSeq.create (3 * v nlimb) (u64 0)))
-    //point_inv h1 f /\
-    //point_as_nat3_proj h1 f == (S.zero, S.zero, S.zero))
+    stack_allocated f h0 h1 (LSeq.create (3 * v 5ul) (u64 0)))
 
 let create_point () =
-  create (3ul *! nlimb) (u64 0)
+  create (3ul *! 5ul) (u64 0)
 
 
 ///  Conversion functions between affine and projective coordinates
 
 inline_for_extraction noextract
-let as_nat_be (h:mem) (b:lbuffer uint8 32ul) =
-  BSeq.nat_from_bytes_be (as_seq h b)
-
-
-inline_for_extraction noextract
 val to_proj_point (p:point) (x y:felem) : Stack unit
   (requires fun h ->
     live h p /\ live h x /\ live h y /\ disjoint p x /\ disjoint p y /\
-    fe_lt_prime h x /\ fe_lt_prime h y)
+    inv_lazy_reduced2 h x /\ inv_lazy_reduced2 h y)
   (ensures  fun h0 _ h1 -> modifies (loc p) h0 h1 /\ point_inv h1 p /\
-    point_as_nat3_proj h1 p == (as_nat h0 x, as_nat h0 y, S.one))
+    point_nat h1 p == (as_nat h0 x, as_nat h0 y, S.one))
 
 let to_proj_point p x y =
   let x1, y1, z1 = getx p, gety p, getz p in
@@ -121,7 +116,7 @@ let to_proj_point p x y =
 inline_for_extraction noextract
 val is_on_curve_vartime (x y:felem) : Stack bool
   (requires fun h -> live h x /\ live h y /\
-    fe_lt_prime h x /\ fe_lt_prime h y)
+    inv_fully_reduced h x /\ inv_fully_reduced h y)
   (ensures  fun h0 b h1 -> modifies0 h0 h1 /\
     b == S.is_on_curve (as_nat h0 x, as_nat h0 y))
 
@@ -131,11 +126,32 @@ let is_on_curve_vartime x y =
   let x3 = create_felem () in
   let b = create_felem () in
 
+  let h = ST.get () in
   fsqr y2 y;
   fsqr x3 x;
   fmul x3 x3 x;
-  make_u64_4 b (make_b_k256 ());
+  let h0 = ST.get () in
+  //assert (feval h0 y2 == S.fmul (feval h y) (feval h y));
+  assert (felem_fits5 (as_felem5 h0 y2) (1,1,1,1,2));
+
+  //assert (feval h0 x3 == S.fmul (S.fmul (feval h x) (feval h x)) (feval h x));
+  assert (felem_fits5 (as_felem5 h0 x3) (1,1,1,1,2));
+
+  make_u52_5 b (make_b_k256 ());
+  let h0' = ST.get () in
+  assert (as_nat h0' b == S.b);
+  assert (felem_fits5 (as_felem5 h0' b) (1,1,1,1,1));
+
+  BL.fadd5_lemma (1,1,1,1,2) (1,1,1,1,1) (as_felem5 h0 x3) (as_felem5 h0' b);
   fadd x3 x3 b;
+  let h1 = ST.get () in
+  assert (felem_fits5 (as_felem5 h1 x3) (2,2,2,2,3));
+
+  fnormalize x3 x3;
+  fnormalize y2 y2;
+  BL.normalize5_lemma (2,2,2,2,3) (as_felem5 h1 x3);
+  BL.normalize5_lemma (1,1,1,1,2) (as_felem5 h1 y2);
+
   let res = is_felem_eq_vartime y2 x3 in
   pop_frame ();
   res
@@ -145,7 +161,17 @@ inline_for_extraction noextract
 val is_proj_point_at_inf_vartime: p:point -> Stack bool
   (requires fun h -> live h p /\ point_inv h p)
   (ensures  fun h0 b h1 -> modifies0 h0 h1 /\
-    b = S.is_proj_point_at_inf (point_as_nat3_proj h0 p))
+    b = S.is_proj_point_at_inf (point_eval h0 p))
 
 let is_proj_point_at_inf_vartime p =
-  is_felem_zero_vartime (getz p)
+  push_frame ();
+  let tmp = create_felem () in
+  let pz = getz p in
+
+  let h0 = ST.get () in
+  assert (inv_lazy_reduced2 h0 (gsub p 10ul 5ul));
+  BL.normalize5_lemma (1,1,1,1,2) (as_felem5 h0 pz);
+  fnormalize tmp pz;
+  let b = is_felem_zero_vartime tmp in
+  pop_frame ();
+  b
