code/k256/Hacl.Impl.K256.PointAdd.fst
@@ -10,7 +10,10 @@ open Lib.Buffer
 module ST = FStar.HyperStack.ST
 module LSeq = Lib.Sequence
 module BSeq = Lib.ByteSequence
+
 module S = Spec.K256
+module BI = Hacl.Spec.K256.Field52
+module BL = Hacl.Spec.K256.Field52.Lemmas
 
 open Hacl.K256.Field
 open Hacl.Impl.K256.Point
@@ -29,34 +32,36 @@ val point_add_xy_pairs (x1 y1 x2 y2 xx yy tmp xy_pairs:felem) : Stack unit
     disjoint xx xy_pairs /\ disjoint yy xy_pairs /\ disjoint xx tmp /\ disjoint yy tmp /\
     disjoint xy_pairs tmp /\
 
-    fe_lt_prime h x1 /\ fe_lt_prime h y1 /\ fe_lt_prime h x2 /\ fe_lt_prime h y2 /\
-    fe_lt_prime h xx /\ fe_lt_prime h yy)
+    inv_lazy_reduced2 h x1 /\ inv_lazy_reduced2 h y1 /\ inv_lazy_reduced2 h x2 /\ inv_lazy_reduced2 h y2 /\
+    inv_lazy_reduced2 h xx /\ inv_lazy_reduced2 h yy)
   (ensures  fun h0 _ h1 -> modifies (loc xy_pairs |+| loc tmp) h0 h1 /\
-    as_nat h1 xy_pairs =
+    feval h1 xy_pairs =
       S.fsub
-	(S.fmul (S.fadd (as_nat h0 x1) (as_nat h0 y1)) (S.fadd (as_nat h0 x2) (as_nat h0 y2)))
-	(S.fadd (as_nat h0 xx) (as_nat h0 yy)) /\
-    fe_lt_prime h1 xy_pairs)
+	(S.fmul (S.fadd (feval h0 x1) (feval h0 y1)) (S.fadd (feval h0 x2) (feval h0 y2)))
+	(S.fadd (feval h0 xx) (feval h0 yy)) /\
+    felem_fits5 (as_felem5 h1 xy_pairs) (9,9,9,9,10))
 
 let point_add_xy_pairs x1 y1 x2 y2 xx yy tmp xy_pairs =
-  //let h0 = ST.get () in
+  let h0 = ST.get () in
+  BL.fadd5_lemma (1,1,1,1,2) (1,1,1,1,2) (as_felem5 h0 x1) (as_felem5 h0 y1);
+  BL.fadd5_lemma (1,1,1,1,2) (1,1,1,1,2) (as_felem5 h0 x2) (as_felem5 h0 y2);
   fadd xy_pairs x1 y1;
   fadd tmp x2 y2;
-  //let h1 = ST.get () in
-  //assert (as_nat h1 xy_pairs == S.fadd (as_nat h0 x1) (as_nat h0 y1));
-  //assert (as_nat h1 tmp == S.fadd (as_nat h0 x2) (as_nat h0 y2));
+  let h1 = ST.get () in
+  assert (felem_fits5 (as_felem5 h1 xy_pairs) (2,2,2,2,4));
+  assert (felem_fits5 (as_felem5 h1 tmp) (2,2,2,2,4));
   fmul xy_pairs xy_pairs tmp;
+  let h2 = ST.get () in
+  assert (felem_fits5 (as_felem5 h2 xy_pairs) (1,1,1,1,2));
+  BL.fadd5_lemma (1,1,1,1,2) (1,1,1,1,2) (as_felem5 h2 xx) (as_felem5 h2 yy);
   fadd tmp xx yy;
-  //let h2 = ST.get () in
-  //assert (as_nat h2 xy_pairs == S.fmul (as_nat h1 xy_pairs) (as_nat h1 tmp));
-  //assert (as_nat h2 tmp = S.fadd (as_nat h0 xx) (as_nat h0 yy));
-  fsub xy_pairs xy_pairs tmp
-  //let h3 = ST.get () in
-  //assert (as_nat h3 xy_pairs == S.fsub (as_nat h2 xy_pairs) (as_nat h2 tmp));
-  //assert (as_nat h3 xy_pairs ==
-    // S.fsub
-    //   (S.fmul (S.fadd (as_nat h0 x1) (as_nat h0 y1)) (S.fadd (as_nat h0 x2) (as_nat h0 y2)))
-    //   (S.fadd (as_nat h0 xx) (as_nat h0 yy)))
+  let h3 = ST.get () in
+  assert (felem_fits5 (as_felem5 h3 tmp) (2,2,2,2,4));
+
+  fsub xy_pairs xy_pairs tmp (u64 4);
+  let h4 = ST.get () in
+  BL.fsub5_lemma (1,1,1,1,2) (2,2,2,2,4) (as_felem5 h3 xy_pairs) (as_felem5 h3 tmp) (u64 4);
+  assert (felem_fits5 (as_felem5 h4 xy_pairs) (9,9,9,9,10))
 
 
 inline_for_extraction noextract
@@ -66,18 +71,29 @@ val ab_plus_cd (a b c d tmp:felem) : Stack unit
     disjoint a b /\ disjoint c d /\ eq_or_disjoint a b /\ eq_or_disjoint a d /\
     disjoint a tmp /\ disjoint b tmp /\ disjoint c tmp /\ disjoint d tmp /\
 
-    fe_lt_prime h a /\ fe_lt_prime h b /\ fe_lt_prime h c /\ fe_lt_prime h d)
+    felem_fits5 (as_felem5 h a) (9,9,9,9,10) /\
+    felem_fits5 (as_felem5 h b) (5,5,5,5,6) /\
+    felem_fits5 (as_felem5 h c) (3,3,3,3,6) /\
+    felem_fits5 (as_felem5 h d) (9,9,9,9,10))
   (ensures fun h0 _ h1 -> modifies (loc c |+| loc tmp) h0 h1 /\
-    as_nat h1 c ==
+    feval h1 c ==
       S.fadd
-	(S.fmul (as_nat h0 a) (as_nat h0 b))
-	(S.fmul (as_nat h0 c) (as_nat h0 d)) /\
-    fe_lt_prime h1 c)
+	(S.fmul (feval h0 a) (feval h0 b))
+	(S.fmul (feval h0 c) (feval h0 d)) /\
+    inv_lazy_reduced2 h1 c)
 
 let ab_plus_cd a b c d tmp =
   fmul tmp a b;
   fmul c c d;
-  fadd c tmp c
+  let h1 = ST.get () in
+  assert (inv_lazy_reduced2 h1 tmp);
+  assert (inv_lazy_reduced2 h1 c);
+  BL.fadd5_lemma (1,1,1,1,2) (1,1,1,1,2) (as_felem5 h1 tmp) (as_felem5 h1 c);
+  fadd c tmp c;
+  let h2 = ST.get () in
+  assert (felem_fits5 (as_felem5 h2 c) (2,2,2,2,4));
+  fnormalize_weak c c;
+  BL.normalize_weak5_lemma (2,2,2,2,4) (as_felem5 h2 c)
 
 
 inline_for_extraction noextract
@@ -87,19 +103,32 @@ val ab_minus_cd (a b c d tmp:felem) : Stack unit
     disjoint a b /\ disjoint c d /\ eq_or_disjoint a b /\ eq_or_disjoint a d /\
     disjoint a tmp /\ disjoint b tmp /\ disjoint c tmp /\ disjoint d tmp /\
 
-    fe_lt_prime h a /\ fe_lt_prime h b /\ fe_lt_prime h c /\ fe_lt_prime h d)
+    felem_fits5 (as_felem5 h a) (9,9,9,9,10) /\
+    felem_fits5 (as_felem5 h b) (5,5,5,5,6) /\
+    felem_fits5 (as_felem5 h c) (1,1,1,1,2) /\
+    felem_fits5 (as_felem5 h d) (9,9,9,9,10))
   (ensures fun h0 _ h1 -> modifies (loc c |+| loc tmp) h0 h1 /\
-    as_nat h1 c ==
+    feval h1 c ==
       S.fsub
-	(S.fmul (as_nat h0 a) (as_nat h0 b))
-	(S.fmul (as_nat h0 c) (as_nat h0 d)) /\
-    fe_lt_prime h1 c)
+	(S.fmul (feval h0 a) (feval h0 b))
+	(S.fmul (feval h0 c) (feval h0 d)) /\
+    inv_lazy_reduced2 h1 c)
 
 let ab_minus_cd a b c d tmp =
   fmul tmp a b;
   fmul c c d;
-  fsub c tmp c
+  let h1 = ST.get () in
+  assert (inv_lazy_reduced2 h1 tmp);
+  assert (inv_lazy_reduced2 h1 c);
+  BL.fsub5_lemma (1,1,1,1,2) (1,1,1,1,2) (as_felem5 h1 tmp) (as_felem5 h1 c) (u64 2);
+  fsub c tmp c (u64 2);
+  let h2 = ST.get () in
+  assert (felem_fits5 (as_felem5 h2 c) (5,5,5,5,6));
+  fnormalize_weak c c;
+  BL.normalize_weak5_lemma (5,5,5,5,6) (as_felem5 h2 c)
 
+
+#set-options "--z3rlimit 300"
 
 inline_for_extraction noextract
 val point_add_no_alloc (out p q:point) (tmp:lbuffer uint64 (9ul *! nlimb)) : Stack unit
@@ -109,7 +138,7 @@ val point_add_no_alloc (out p q:point) (tmp:lbuffer uint64 (9ul *! nlimb)) : Sta
     disjoint p tmp /\ disjoint q tmp /\ disjoint out tmp /\
     point_inv h p /\ point_inv h q)
   (ensures fun h0 _ h1 -> modifies (loc out |+| loc tmp) h0 h1 /\ point_inv h1 out /\
-    point_as_nat3_proj h1 out == S.point_add (point_as_nat3_proj h0 p) (point_as_nat3_proj h0 q))
+    point_eval h1 out == S.point_add (point_eval h0 p) (point_eval h0 q))
 
 let point_add_no_alloc out p q tmp =
   let x1, y1, z1 = getx p, gety p, getz p in
@@ -133,69 +162,49 @@ let point_add_no_alloc out p q tmp =
   fmul xx x1 x2; //xx = x1*x2
   fmul yy y1 y2; //yy = y1*y2
   fmul zz z1 z2; //zz = z1*z2
-
-  // let h1 = ST.get () in
-  // assert (as_nat h1 xx == S.fmul (as_nat h0 x1) (as_nat h0 x2));
-  // assert (as_nat h1 yy == S.fmul (as_nat h0 y1) (as_nat h0 y2));
-  // assert (as_nat h1 zz == S.fmul (as_nat h0 z1) (as_nat h0 z2));
+  let h1 = ST.get () in
+  // assert (inv_lazy_reduced2 h1 xx);
+  // assert (inv_lazy_reduced2 h1 yy);
+  // assert (inv_lazy_reduced2 h1 zz);
 
   point_add_xy_pairs x1 y1 x2 y2 xx yy tmp1 xy_pairs; //xy_pairs = (x1+y1)*(x2+y2)-(xx+yy)
   point_add_xy_pairs y1 z1 y2 z2 yy zz tmp1 yz_pairs; //yz_pairs = (y1+z1)*(y2+z2)-(yy+zz)
   point_add_xy_pairs x1 z1 x2 z2 xx zz tmp1 xz_pairs; //xz_pairs = (x1+z1)*(x2+z2)-(xx+zz)
 
-  // let h2 = ST.get () in
-  // assert (as_nat h2 xy_pairs ==
-  //   S.fsub
-  //     (S.fmul (S.fadd (as_nat h0 x1) (as_nat h0 y1)) (S.fadd (as_nat h0 x2) (as_nat h0 y2)))
-  //     (S.fadd (as_nat h1 xx) (as_nat h1 yy)));
+  let h2 = ST.get () in
+  // assert (felem_fits5 (as_felem5 h2 xy_pairs) (9,9,9,9,10));
+  // assert (felem_fits5 (as_felem5 h2 yz_pairs) (9,9,9,9,10));
+  // assert (felem_fits5 (as_felem5 h2 xz_pairs) (9,9,9,9,10));
 
-  // assert (as_nat h2 yz_pairs ==
-  //   S.fsub
-  //     (S.fmul (S.fadd (as_nat h0 y1) (as_nat h0 z1)) (S.fadd (as_nat h0 y2) (as_nat h0 z2)))
-  //     (S.fadd (as_nat h1 yy) (as_nat h1 zz)));
+  fmul_3b_normalize_weak tmp1 zz; //tmp1 = bzz3 = (3*b)*zz
+  let h3 = ST.get () in
+  // assert (felem_fits5 (as_felem5 h3 tmp1) (1,1,1,1,2));
 
-  // assert (as_nat h2 xz_pairs ==
-  //   S.fsub
-  //     (S.fmul (S.fadd (as_nat h0 x1) (as_nat h0 z1)) (S.fadd (as_nat h0 x2) (as_nat h0 z2)))
-  //     (S.fadd (as_nat h1 xx) (as_nat h1 zz)));
+  fsub yy_m_bzz3 yy tmp1 (u64 2); //yy_m_bzz3 = yy-bzz3
+  let h5 = ST.get () in
+  BL.fsub5_lemma (1,1,1,1,2) (1,1,1,1,2) (as_felem5 h3 yy) (as_felem5 h3 tmp1) (u64 2);
+  // assert (felem_fits5 (as_felem5 h5 yy_m_bzz3) (5,5,5,5,6));
 
-  fmul_3b tmp1 zz; //tmp1 = bzz3 = (3*b)*zz
-  fsub yy_m_bzz3 yy tmp1; //yy_m_bzz3 = yy-bzz3
   fadd yy_p_bzz3 yy tmp1; //yy_p_bzz3 = yy+bzz3
+  let h6 = ST.get () in
+  BL.fadd5_lemma (1,1,1,1,2) (1,1,1,1,2) (as_felem5 h3 yy) (as_felem5 h3 tmp1);
+  // assert (felem_fits5 (as_felem5 h6 yy_p_bzz3) (2,2,2,2,4));
 
-  // let h3 = ST.get () in
-  // assert (as_nat h3 tmp1 = S.fmul (S.fmul 3 S.b) (as_nat h1 zz));
-  // assert (as_nat h3 yy_m_bzz3 = S.fsub (as_nat h1 yy) (as_nat h3 tmp1));
-  // assert (as_nat h3 yy_p_bzz3 = S.fadd (as_nat h1 yy) (as_nat h3 tmp1));
+  fmul_3b_normalize_weak x3 yz_pairs; //x3 = byz3 = (3*b)*yz_pairs
+  let h7 = ST.get () in
+  // assert (felem_fits5 (as_felem5 h7 x3) (1,1,1,1,2));
 
-  fmul_3b x3 yz_pairs; //x3 = byz3 = (3*b)*yz_pairs
   fmul_small_num z3 xx (u64 3); //z3 = xx3 = 3*xx
-  fmul_3b y3 z3; //y3 = bxx9 = (3*b)*xx3
+  let h8 = ST.get () in
+  BL.fmul15_lemma (1,1,1,1,2) 3 (as_felem5 h7 xx) (u64 3);
+  // assert (felem_fits5 (as_felem5 h8 z3) (3,3,3,3,6));
 
-  // let h4 = ST.get () in
-  // assert (as_nat h4 x3 = S.fmul (S.fmul 3 S.b) (as_nat h2 yz_pairs));
-  // assert (as_nat h4 z3 = S.fmul 3 (as_nat h1 xx));
-  // assert (as_nat h4 y3 = S.fmul (S.fmul 3 S.b) (as_nat h4 z3));
-
+  fmul_3b_normalize_weak y3 z3; //y3 = bxx9 = (3*b)*xx3
+  let h9 = ST.get () in
+  // assert (felem_fits5 (as_felem5 h9 y3) (1,1,1,1,2));
   ab_minus_cd xy_pairs yy_m_bzz3 x3 xz_pairs tmp1; //x3 = (xy_pairs*yy_m_bzz3-byz3*xz_pairs)
   ab_plus_cd yy_p_bzz3 yy_m_bzz3 y3 xz_pairs tmp1; //y3 = (yy_p_bzz3*yy_m_bzz3+bxx9*xz_pairs)
   ab_plus_cd yz_pairs yy_p_bzz3 z3 xy_pairs tmp1 //z3 = (yz_pairs*yy_p_bzz3+xx3*xy_pairs)
-
-  // let h5 = ST.get () in
-  // assert (as_nat h5 x3 =
-  //   S.fsub
-  //     (S.fmul (as_nat h2 xy_pairs) (as_nat h3 yy_m_bzz3))
-  //     (S.fmul (as_nat h4 x3) (as_nat h2 xz_pairs)));
-
-  // assert (as_nat h5 y3 =
-  //   S.fadd
-  //     (S.fmul (as_nat h3 yy_p_bzz3) (as_nat h3 yy_m_bzz3))
-  //     (S.fmul (as_nat h4 y3) (as_nat h2 xz_pairs)));
-
-  // assert (as_nat h5 z3 =
-  //   S.fadd
-  //     (S.fmul (as_nat h2 yz_pairs) (as_nat h3 yy_p_bzz3))
-  //     (S.fmul (as_nat h4 z3) (as_nat h2 xy_pairs)))
 
 
 val point_add (out p q:point) : Stack unit
@@ -204,7 +213,7 @@ val point_add (out p q:point) : Stack unit
     eq_or_disjoint out p /\ eq_or_disjoint out q /\ eq_or_disjoint p q /\
     point_inv h p /\ point_inv h q)
   (ensures fun h0 _ h1 -> modifies (loc out) h0 h1 /\ point_inv h1 out /\
-    point_as_nat3_proj h1 out == S.point_add (point_as_nat3_proj h0 p) (point_as_nat3_proj h0 q))
+    point_eval h1 out == S.point_add (point_eval h0 p) (point_eval h0 q))
 
 [@CInline]
 let point_add out p q =
