code/k256/Hacl.Impl.K256.PointDouble.fst
@@ -10,12 +10,15 @@ open Lib.Buffer
 module ST = FStar.HyperStack.ST
 module LSeq = Lib.Sequence
 module BSeq = Lib.ByteSequence
+
 module S = Spec.K256
+module BI = Hacl.Spec.K256.Field52
+module BL = Hacl.Spec.K256.Field52.Lemmas
 
 open Hacl.K256.Field
 open Hacl.Impl.K256.Point
 
-#set-options "--z3rlimit 100 --fuel 0 --ifuel 0"
+#set-options "--z3rlimit 300 --fuel 0 --ifuel 0"
 
 
 inline_for_extraction noextract
@@ -25,7 +28,7 @@ val point_double_no_alloc (out p:point) (tmp:lbuffer uint64 (5ul *! nlimb)) : St
     eq_or_disjoint out p /\ disjoint out tmp /\ disjoint p tmp /\
     point_inv h p)
   (ensures fun h0 _ h1 -> modifies (loc out |+| loc tmp) h0 h1 /\ point_inv h1 out /\
-    point_as_nat3_proj h1 out == S.point_double (point_as_nat3_proj h0 p))
+    point_eval h1 out == S.point_double (point_eval h0 p))
 
 let point_double_no_alloc out p tmp =
   let x1, y1, z1 = getx p, gety p, getz p in
@@ -37,29 +40,68 @@ let point_double_no_alloc out p tmp =
   let bzz9 = sub tmp (3ul *! nlimb) nlimb in
   let tmp = sub tmp (4ul *! nlimb) nlimb in
 
+  let h0 = ST.get () in
   fsqr yy y1; //yy = y*y
   fsqr zz z1; //zz = z*z
+  let h1 = ST.get () in
+  //assert (inv_lazy_reduced2 h1 yy);
+  //assert (inv_lazy_reduced2 h1 zz);
 
   fmul_small_num x3 x1 (u64 2); //x3 = 2*x
-  fmul x3 x3 y1; //x3 = xy2 = x3*y = (2*x)*y
+  let h2 = ST.get () in
+  BL.fmul15_lemma (1,1,1,1,2) 2 (as_felem5 h1 x1) (u64 2);
+  //assert (felem_fits5 (as_felem5 h2 x3) (2,2,2,2,4));
 
+  fmul x3 x3 y1; //x3 = xy2 = x3*y = (2*x)*y
   fmul tmp yy y1; //tmp = yy*y
   fmul z3 tmp z1; //z3 = tmp*z = yy*y*z
-  fmul_small_num z3 z3 (u64 8); //z3 = z3*8=yy*y*z*8
+  let h3 = ST.get () in
+  //assert (inv_lazy_reduced2 h3 x3);
+  //assert (inv_lazy_reduced2 h3 tmp);
+  //assert (inv_lazy_reduced2 h3 z3);
 
-  fmul_3b bzz3 zz; //bzz3 = (3*b)*zz
+  fmul_8_normalize_weak z3 z3; //z3 = z3*8=yy*y*z*8
+  fmul_3b_normalize_weak bzz3 zz; //bzz3 = (3*b)*zz
+  let h5 = ST.get () in
+  //assert (inv_lazy_reduced2 h5 z3);
+  //assert (inv_lazy_reduced2 h5 bzz3);
+
   fmul_small_num bzz9 bzz3 (u64 3); //bzz9 = 3*bzz3
+  let h6 = ST.get () in
+  BL.fmul15_lemma (1,1,1,1,2) 3 (as_felem5 h5 bzz3) (u64 3);
+  //assert (felem_fits5 (as_felem5 h6 bzz9) (3,3,3,3,6));
 
-  fsub bzz9 yy bzz9; //bzz9 = yy_m_bzz9 = yy-bzz9
+  BL.fsub5_lemma (1,1,1,1,2) (3,3,3,3,6) (as_felem5 h6 yy) (as_felem5 h6 bzz9) (u64 6);
+  fsub bzz9 yy bzz9 (u64 6); //bzz9 = yy_m_bzz9 = yy-bzz9
+  let h7 = ST.get () in
+  //assert (felem_fits5 (as_felem5 h7 bzz9) (13,13,13,13,14));
+
   fadd tmp yy bzz3; //tmp = yy_p_bzz3 = yy+bzz3
+  let h8 = ST.get () in
+  BL.fadd5_lemma (1,1,1,1,2) (1,1,1,1,2) (as_felem5 h7 yy) (as_felem5 h7 bzz3);
+  //assert (felem_fits5 (as_felem5 h8 tmp) (2,2,2,2,4));
 
   fmul y3 yy zz; //y3 = yy_zz = yy*zz
-  fmul_24b y3 y3; //y3 = t = (24*b)*y3 = (24*b)*yy_zz
+  let h9 = ST.get () in
+  //assert (inv_lazy_reduced2 h9 y3);
+
+  fmul_small_num y3 y3 (u64 168); //y3 = t = (24*b)*y3 = (24*b)*yy_zz
+  let h10 = ST.get () in
+  BL.fmul15_lemma (1,1,1,1,2) 168 (as_felem5 h9 y3) (u64 168);
+  //assert (felem_fits5 (as_felem5 h10 y3) (168,168,168,168,336));
 
   fmul x3 x3 bzz9; //x3 = x3*bzz9 = xy2*yy_m_bzz9
-
   fmul tmp bzz9 tmp; //tmp = bzz9*tmp = yy_m_bzz9*yy_p_bzz3
-  fadd y3 tmp y3  //y3 = tmp+y3 = yy_m_bzz9*yy_p_bzz3+t
+  let h11 = ST.get () in
+  //assert (inv_lazy_reduced2 h11 x3);
+  //assert (inv_lazy_reduced2 h11 tmp);
+
+  fadd y3 tmp y3;  //y3 = tmp+y3 = yy_m_bzz9*yy_p_bzz3+t
+  let h12 = ST.get () in
+  BL.fadd5_lemma (1,1,1,1,2) (168,168,168,168,336) (as_felem5 h11 tmp) (as_felem5 h11 y3);
+  //assert (felem_fits5 (as_felem5 h12 y3) (169,169,169,169,338));
+  fnormalize_weak y3 y3;
+  BL.normalize_weak5_lemma (169,169,169,169,338) (as_felem5 h12 y3)
 
 
 val point_double (out p:point) : Stack unit
@@ -67,7 +109,7 @@ val point_double (out p:point) : Stack unit
     live h out /\ live h p /\ eq_or_disjoint out p /\
     point_inv h p)
   (ensures fun h0 _ h1 -> modifies (loc out) h0 h1 /\ point_inv h1 out /\
-    point_as_nat3_proj h1 out == S.point_double (point_as_nat3_proj h0 p))
+    point_eval h1 out == S.point_double (point_eval h0 p))
 
 [@CInline]
 let point_double out p =
