code/k256/Hacl.Impl.K256.PointMul.fst
@@ -16,11 +16,6 @@ module SE = Spec.Exponentiation
 module BE = Hacl.Impl.Exponentiation
 module ME = Hacl.Impl.MultiExponentiation
 
-module BD = Hacl.Bignum.Definitions
-module SD = Hacl.Spec.Bignum.Definitions
-module BC = Hacl.Bignum.Convert
-module SC = Hacl.Spec.Bignum.Convert
-
 module S = Spec.K256
 
 open Hacl.K256.Field
@@ -35,11 +30,11 @@ unfold
 let linv_ctx (a:LSeq.lseq uint64 0) : Type0 = True
 
 unfold
-let refl (p:LSeq.lseq uint64 12{point_inv_lseq p}) : GTot S.proj_point =
-  point_as_nat3_proj_lseq p
+let refl (p:LSeq.lseq uint64 15{point_inv_lseq p}) : GTot S.proj_point =
+  point_eval_lseq p
 
 inline_for_extraction noextract
-let mk_to_k256_concrete_ops : BE.to_concrete_ops U64 12ul 0ul = {
+let mk_to_k256_concrete_ops : BE.to_concrete_ops U64 15ul 0ul = {
   BE.t_spec = S.proj_point;
   BE.concr_ops = S.mk_k256_concrete_ops;
   BE.linv_ctx = linv_ctx;
@@ -49,19 +44,19 @@ let mk_to_k256_concrete_ops : BE.to_concrete_ops U64 12ul 0ul = {
 
 
 inline_for_extraction noextract
-val point_add : BE.lmul_st U64 12ul 0ul mk_to_k256_concrete_ops
+val point_add : BE.lmul_st U64 15ul 0ul mk_to_k256_concrete_ops
 let point_add ctx x y xy =
   Hacl.Impl.K256.PointAdd.point_add xy x y
 
 
 inline_for_extraction noextract
-val point_double : BE.lsqr_st U64 12ul 0ul mk_to_k256_concrete_ops
+val point_double : BE.lsqr_st U64 15ul 0ul mk_to_k256_concrete_ops
 let point_double ctx x xx =
   Hacl.Impl.K256.PointDouble.point_double xx x
 
 
 inline_for_extraction noextract
-let mk_k256_concrete_ops : BE.concrete_ops U64 12ul 0ul = {
+let mk_k256_concrete_ops : BE.concrete_ops U64 15ul 0ul = {
   BE.to = mk_to_k256_concrete_ops;
   BE.lmul = point_add;
   BE.lsqr = point_double;
@@ -73,7 +68,7 @@ inline_for_extraction noextract
 val make_point_at_inf: p:point -> Stack unit
   (requires fun h -> live h p)
   (ensures  fun h0 _ h1 -> modifies (loc p) h0 h1 /\
-    point_inv h1 p /\ point_as_nat3_proj h1 p == S.point_at_inf)
+    point_inv h1 p /\ point_eval h1 p == S.point_at_inf)
 
 let make_point_at_inf p =
   let px, py, pz = getx p, gety p, getz p in
@@ -87,30 +82,34 @@ val make_g: g:point -> Stack unit
   (requires fun h -> live h g)
   (ensures  fun h0 _ h1 -> modifies (loc g) h0 h1 /\
     point_inv h1 g /\
-    point_as_nat3_proj h1 g == S.g)
+    point_eval h1 g == S.g)
 
 let make_g g =
   let gx, gy, gz = getx g, gety g, getz g in
 
   [@inline_let]
   let x =
-   (u64 0x59f2815b16f81798,
-    u64 0x029bfcdb2dce28d9,
-    u64 0x55a06295ce870b07,
-    u64 0x79be667ef9dcbbac) in
+   (u64 0x2815b16f81798,
+    u64 0xdb2dce28d959f,
+    u64 0xe870b07029bfc,
+    u64 0xbbac55a06295c,
+    u64 0x79be667ef9dc) in
 
-  assert_norm (S.g_x == as_nat4 x);
-  make_u64_4 gx x;
+  assert_norm (0x79be667ef9dc < max48);
+  assert_norm (0xe1108a8fd17b4 < max52);
+  assert_norm (S.g_x == as_nat5 x);
+  make_u52_5 gx x;
 
   [@inline_let]
   let y =
-   (u64 0x9c47d08ffb10d4b8,
-    u64 0xfd17b448a6855419,
-    u64 0x5da4fbfc0e1108a8,
-    u64 0x483ada7726a3c465) in
+   (u64 0x7d08ffb10d4b8,
+    u64 0x48a68554199c4,
+    u64 0xe1108a8fd17b4,
+    u64 0xc4655da4fbfc0,
+    u64 0x483ada7726a3) in
 
-  assert_norm (S.g_y == as_nat4 y);
-  make_u64_4 gy y;
+  assert_norm (S.g_y == as_nat5 y);
+  make_u52_5 gy y;
 
   set_one gz
 
@@ -123,13 +122,12 @@ val point_mul: out:point -> scalar:qelem -> q:point -> Stack unit
     point_inv h q /\ qas_nat h scalar < S.q)
   (ensures  fun h0 _ h1 -> modifies (loc out) h0 h1 /\
     point_inv h1 out /\
-    point_as_nat3_proj h1 out ==
-    S.point_mul (qas_nat h0 scalar) (point_as_nat3_proj h0 q))
+    point_eval h1 out == S.point_mul (qas_nat h0 scalar) (point_eval h0 q))
 
 [@CInline]
 let point_mul out scalar q =
   make_point_at_inf out;
-  BE.lexp_fw_consttime 12ul 0ul mk_k256_concrete_ops (null uint64) q 4ul 256ul scalar out 4ul
+  BE.lexp_fw_consttime 15ul 0ul mk_k256_concrete_ops (null uint64) q 4ul 256ul scalar out 4ul
 
 
 val point_mul_double_vartime:
@@ -142,15 +140,15 @@ val point_mul_double_vartime:
     qas_nat h scalar1 < S.q /\ qas_nat h scalar2 < S.q)
   (ensures fun h0 _ h1 -> modifies (loc out) h0 h1 /\
     point_inv h1 out /\
-    point_as_nat3_proj h1 out ==
+    point_eval h1 out ==
     S.point_mul_double
-      (qas_nat h0 scalar1) (point_as_nat3_proj h0 q1)
-      (qas_nat h0 scalar2) (point_as_nat3_proj h0 q2))
+      (qas_nat h0 scalar1) (point_eval h0 q1)
+      (qas_nat h0 scalar2) (point_eval h0 q2))
 
 [@CInline]
 let point_mul_double_vartime out scalar1 q1 scalar2 q2 =
   make_point_at_inf out;
-  ME.lexp_double_fw_vartime 12ul 0ul mk_k256_concrete_ops (null uint64) q1 4ul 256ul scalar1 q2 scalar2 out 4ul
+  ME.lexp_double_fw_vartime 15ul 0ul mk_k256_concrete_ops (null uint64) q1 4ul 256ul scalar1 q2 scalar2 out 4ul
 
 
 val point_mul_g: out:point -> scalar:qelem -> Stack unit
@@ -159,12 +157,12 @@ val point_mul_g: out:point -> scalar:qelem -> Stack unit
     qas_nat h scalar < S.q)
   (ensures  fun h0 _ h1 -> modifies (loc out) h0 h1 /\
     point_inv h1 out /\
-    point_as_nat3_proj h1 out == S.point_mul_g (qas_nat h0 scalar))
+    point_eval h1 out == S.point_mul_g (qas_nat h0 scalar))
 
 [@CInline]
 let point_mul_g out scalar =
   push_frame ();
-  let g = create 12ul (u64 0) in
+  let g = create 15ul (u64 0) in
   make_g g;
   point_mul out scalar g;
   pop_frame ()
@@ -178,14 +176,14 @@ val point_mul_g_double_vartime: out:point -> scalar1:qelem -> scalar2:qelem -> q
     point_inv h q2 /\ qas_nat h scalar1 < S.q /\ qas_nat h scalar2 < S.q)
   (ensures fun h0 _ h1 -> modifies (loc out) h0 h1 /\
     point_inv h1 out /\
-    point_as_nat3_proj h1 out ==
+    point_eval h1 out ==
     S.point_mul_double_g
-      (qas_nat h0 scalar1) (qas_nat h0 scalar2) (point_as_nat3_proj h0 q2))
+      (qas_nat h0 scalar1) (qas_nat h0 scalar2) (point_eval h0 q2))
 
 [@CInline]
 let point_mul_g_double_vartime out scalar1 scalar2 q2 =
   push_frame ();
-  let g = create 12ul (u64 0) in
+  let g = create 15ul (u64 0) in
   make_g g;
   point_mul_double_vartime out scalar1 g scalar2 q2;
   pop_frame ()
