code/k256/Hacl.Spec.K256.Field52.Lemmas3.fst
@@ -43,59 +43,59 @@ let lemma_bound_mul64_wide ma mb mma mmb a b =
 
 val lemma_four_mul64_wide (a0 a1 a2 a3 b0 b1 b2 b3:uint64) : Lemma
   (requires
-    felem_fits1 a0 8 /\ felem_fits1 b0 8 /\
-    felem_fits1 a1 8 /\ felem_fits1 b1 8 /\
-    felem_fits1 a2 8 /\ felem_fits1 b2 8 /\
-    felem_fits1 a3 8 /\ felem_fits1 b3 8)
+    felem_fits1 a0 64 /\ felem_fits1 b0 64 /\
+    felem_fits1 a1 64 /\ felem_fits1 b1 64 /\
+    felem_fits1 a2 64 /\ felem_fits1 b2 64 /\
+    felem_fits1 a3 64 /\ felem_fits1 b3 64)
   (ensures
    (let d = mul64_wide a0 b3 +. mul64_wide a1 b2 +. mul64_wide a2 b1 +. mul64_wide a3 b0 in
     v d = v a0 * v b3 + v a1 * v b2 + v a2 * v b1 + v a3 * v b0 /\
-    v d <= 256 * (max52 * max52)))
+    v d <= 16384 * (max52 * max52)))
 
 let lemma_four_mul64_wide a0 a1 a2 a3 b0 b1 b2 b3 =
-  lemma_bound_mul64_wide 8 8 max52 max52 a0 b3;
-  lemma_bound_mul64_wide 8 8 max52 max52 a1 b2;
-  lemma_bound_mul64_wide 8 8 max52 max52 a2 b1;
-  lemma_bound_mul64_wide 8 8 max52 max52 a3 b0;
-  assert (v a0 * v b3 + v a1 * v b2 + v a2 * v b1 + v a3 * v b0 <= 256 * (max52 * max52));
-  assert_norm (256 * (max52 * max52) < pow2 128);
+  lemma_bound_mul64_wide 64 64 max52 max52 a0 b3;
+  lemma_bound_mul64_wide 64 64 max52 max52 a1 b2;
+  lemma_bound_mul64_wide 64 64 max52 max52 a2 b1;
+  lemma_bound_mul64_wide 64 64 max52 max52 a3 b0;
+  assert (v a0 * v b3 + v a1 * v b2 + v a2 * v b1 + v a3 * v b0 <= 16384 * (max52 * max52));
+  assert_norm (16384 * (max52 * max52) < pow2 128);
 
   Math.Lemmas.small_mod (v a0 * v b3 + v a1 * v b2) (pow2 128);
   Math.Lemmas.small_mod (v a0 * v b3 + v a1 * v b2 + v a2 * v b1) (pow2 128);
   Math.Lemmas.small_mod (v a0 * v b3 + v a1 * v b2 + v a2 * v b1 + v a3 * v b0) (pow2 128)
 
 
-val lemma_128_max52_max48: unit -> Lemma (128 * (max52 * max48) < 8 * (max52 * max52))
-let lemma_128_max52_max48 () =
-  assert_norm (128 * (max52 * max48) < 8 * (max52 * max52))
+val lemma_16_max52_max48: unit -> Lemma (16 * (max52 * max48) < max52 * max52)
+let lemma_16_max52_max48 () =
+  assert_norm (16 * (max52 * max48) < max52 * max52)
 
 
 val lemma_add_five_mul64_wide (md:nat) (d:uint128) (a0 a1 a2 a3 a4 b0 b1 b2 b3 b4:uint64) : Lemma
   (requires
-    v d <= md * max52 /\ md <= 321 /\
-    felem_fits1 a0 8 /\ felem_fits1 b0 8 /\
-    felem_fits1 a1 8 /\ felem_fits1 b1 8 /\
-    felem_fits1 a2 8 /\ felem_fits1 b2 8 /\
-    felem_fits1 a3 8 /\ felem_fits1 b3 8 /\
-    felem_fits_last1 a4 8 /\ felem_fits_last1 b4 8)
+    v d <= md * max52 /\ md <= 16385 /\
+    felem_fits1 a0 64 /\ felem_fits1 b0 64 /\
+    felem_fits1 a1 64 /\ felem_fits1 b1 64 /\
+    felem_fits1 a2 64 /\ felem_fits1 b2 64 /\
+    felem_fits1 a3 64 /\ felem_fits1 b3 64 /\
+    felem_fits_last1 a4 64 /\ felem_fits_last1 b4 64)
   (ensures
    (let d1 = d +. mul64_wide a0 b4 +. mul64_wide a1 b3 +.
      mul64_wide a2 b2 +. mul64_wide a3 b1 +. mul64_wide a4 b0 in
     v d1 == v d + v a0 * v b4 + v a1 * v b3 + v a2 * v b2 + v a3 * v b1 + v a4 * v b0 /\
-    v d1 <= 201 * (max52 * max52)))
+    v d1 <= 12801 * (max52 * max52)))
 
 let lemma_add_five_mul64_wide md d a0 a1 a2 a3 a4 b0 b1 b2 b3 b4 =
-  lemma_bound_mul64_wide 8 8 max52 max48 a0 b4;
-  lemma_bound_mul64_wide 8 8 max52 max52 a1 b3;
-  lemma_bound_mul64_wide 8 8 max52 max52 a2 b2;
-  lemma_bound_mul64_wide 8 8 max52 max52 a3 b1;
-  lemma_bound_mul64_wide 8 8 max48 max52 a4 b0;
+  lemma_bound_mul64_wide 64 64 max52 max48 a0 b4;
+  lemma_bound_mul64_wide 64 64 max52 max52 a1 b3;
+  lemma_bound_mul64_wide 64 64 max52 max52 a2 b2;
+  lemma_bound_mul64_wide 64 64 max52 max52 a3 b1;
+  lemma_bound_mul64_wide 64 64 max48 max52 a4 b0;
   Math.Lemmas.swap_mul max52 max48;
   assert (v d + v a0 * v b4 + v a1 * v b3 + v a2 * v b2 + v a3 * v b1 + v a4 * v b0 <=
-    md * max52 + 128 * (max52 * max48) + 192 * (max52 * max52));
-  lemma_128_max52_max48 ();
-  assert_norm (md * max52 + 128 * (max52 * max48) + 192 * (max52 * max52) <= 201 * (max52 * max52));
-  assert_norm (201 * (max52 * max52) < pow2 128);
+    md * max52 + 8192 * (max52 * max48) + 12288 * (max52 * max52));
+  lemma_16_max52_max48 ();
+  assert_norm (md * max52 + 8192 * (max52 * max48) + 12288 * (max52 * max52) <= 12801 * (max52 * max52));
+  assert_norm (12801 * (max52 * max52) < pow2 128);
 
   Math.Lemmas.small_mod (v d + v a0 * v b4) (pow2 128);
   Math.Lemmas.small_mod (v d + v a0 * v b4 + v a1 * v b3) (pow2 128);
@@ -106,27 +106,27 @@ let lemma_add_five_mul64_wide md d a0 a1 a2 a3 a4 b0 b1 b2 b3 b4 =
 
 val lemma_add_four_mul64_wide (md:nat) (d:uint128) (a1 a2 a3 a4 b1 b2 b3 b4:uint64) : Lemma
   (requires
-    v d <= md * max52 /\ md <= 321 /\
-    felem_fits1 a1 8 /\ felem_fits1 b1 8 /\
-    felem_fits1 a2 8 /\ felem_fits1 b2 8 /\
-    felem_fits1 a3 8 /\ felem_fits1 b3 8 /\
-    felem_fits_last1 a4 8 /\ felem_fits_last1 b4 8)
+    v d <= md * max52 /\ md <= 12802 /\
+    felem_fits1 a1 64 /\ felem_fits1 b1 64 /\
+    felem_fits1 a2 64 /\ felem_fits1 b2 64 /\
+    felem_fits1 a3 64 /\ felem_fits1 b3 64 /\
+    felem_fits_last1 a4 64 /\ felem_fits_last1 b4 64)
   (ensures
    (let d1 = d +. mul64_wide a1 b4 +. mul64_wide a2 b3 +.
      mul64_wide a3 b2 +. mul64_wide a4 b1 in
     v d1 == v d + v a1 * v b4 + v a2 * v b3 + v a3 * v b2 + v a4 * v b1 /\
-    v d1 <= 201 * (max52 * max52)))
+    v d1 <= 8705 * (max52 * max52)))
 
 let lemma_add_four_mul64_wide md d a1 a2 a3 a4 b1 b2 b3 b4 =
-  lemma_bound_mul64_wide 8 8 max52 max48 a1 b4;
-  lemma_bound_mul64_wide 8 8 max52 max52 a2 b3;
-  lemma_bound_mul64_wide 8 8 max52 max52 a3 b2;
-  lemma_bound_mul64_wide 8 8 max48 max52 a4 b1;
+  lemma_bound_mul64_wide 64 64 max52 max48 a1 b4;
+  lemma_bound_mul64_wide 64 64 max52 max52 a2 b3;
+  lemma_bound_mul64_wide 64 64 max52 max52 a3 b2;
+  lemma_bound_mul64_wide 64 64 max48 max52 a4 b1;
   assert (v d + v a1 * v b4 + v a2 * v b3 + v a3 * v b2 + v a4 * v b1 <=
-    md * max52 + 128 * (max52 * max48) + 128 * (max52 * max52));
-  lemma_128_max52_max48 ();
-  assert_norm (md * max52 + 128 * (max52 * max48) + 128 * (max52 * max52) <= 144 * (max52 * max52));
-  assert_norm (144 * (max52 * max52) < pow2 128);
+    md * max52 + 8192 * (max52 * max48) + 8192 * (max52 * max52));
+  lemma_16_max52_max48 ();
+  assert_norm (md * max52 + 8192 * (max52 * max48) + 8192 * (max52 * max52) <= 8705 * (max52 * max52));
+  assert_norm (8705 * (max52 * max52) < pow2 128);
 
   Math.Lemmas.small_mod (v d + v a1 * v b4) (pow2 128);
   Math.Lemmas.small_mod (v d + v a1 * v b4 + v a2 * v b3) (pow2 128);
@@ -136,22 +136,22 @@ let lemma_add_four_mul64_wide md d a1 a2 a3 a4 b1 b2 b3 b4 =
 
 val lemma_add_three_mul64_wide52 (md:nat) (d:uint128) (a0 a1 a2 b0 b1 b2:uint64) : Lemma
   (requires
-    v d <= md * max52 /\ md <= 130 /\
-    felem_fits1 a0 8 /\ felem_fits1 b0 8 /\
-    felem_fits1 a1 8 /\ felem_fits1 b1 8 /\
-    felem_fits1 a2 8 /\ felem_fits1 b2 8)
+    v d <= md * max52 /\ md <= 8194 /\
+    felem_fits1 a0 64 /\ felem_fits1 b0 64 /\
+    felem_fits1 a1 64 /\ felem_fits1 b1 64 /\
+    felem_fits1 a2 64 /\ felem_fits1 b2 64)
   (ensures
    (let d1 = d +. mul64_wide a0 b2 +. mul64_wide a1 b1 +. mul64_wide a2 b0 in
     v d1 == v d + v a0 * v b2 + v a1 * v b1 + v a2 * v b0 /\
-    v d1 <= 193 * (max52 * max52)))
+    v d1 <= 12289 * (max52 * max52)))
 
 let lemma_add_three_mul64_wide52 md d a0 a1 a2 b0 b1 b2 =
-  lemma_bound_mul64_wide 8 8 max52 max52 a0 b2;
-  lemma_bound_mul64_wide 8 8 max52 max52 a1 b1;
-  lemma_bound_mul64_wide 8 8 max52 max52 a2 b0;
-  assert (v d + v a0 * v b2 + v a1 * v b1 + v a2 * v b0 <= md * max52 + 192 * (max52 * max52));
-  assert_norm (md * max52 + 192 * (max52 * max52) <= 193 * (max52 * max52));
-  assert_norm (193 * (max52 * max52) < pow2 128);
+  lemma_bound_mul64_wide 64 64 max52 max52 a0 b2;
+  lemma_bound_mul64_wide 64 64 max52 max52 a1 b1;
+  lemma_bound_mul64_wide 64 64 max52 max52 a2 b0;
+  assert (v d + v a0 * v b2 + v a1 * v b1 + v a2 * v b0 <= md * max52 + 12288 * (max52 * max52));
+  assert_norm (md * max52 + 12288 * (max52 * max52) <= 12289 * (max52 * max52));
+  assert_norm (12289 * (max52 * max52) < pow2 128);
 
   Math.Lemmas.small_mod (v d + v a0 * v b2) (pow2 128);
   Math.Lemmas.small_mod (v d + v a0 * v b2 + v a1 * v b1) (pow2 128);
@@ -160,26 +160,26 @@ let lemma_add_three_mul64_wide52 md d a0 a1 a2 b0 b1 b2 =
 
 val lemma_add_three_mul64_wide (md:nat) (d:uint128) (a2 a3 a4 b2 b3 b4:uint64) : Lemma
   (requires
-    v d <= md * max52 /\ md <= 320 /\
-    felem_fits1 a2 8 /\ felem_fits1 b2 8 /\
-    felem_fits1 a3 8 /\ felem_fits1 b3 8 /\
-    felem_fits_last1 a4 8 /\ felem_fits_last1 b4 8)
+    v d <= md * max52 /\ md <= 8705 /\
+    felem_fits1 a2 64 /\ felem_fits1 b2 64 /\
+    felem_fits1 a3 64 /\ felem_fits1 b3 64 /\
+    felem_fits_last1 a4 64 /\ felem_fits_last1 b4 64)
   (ensures
    (let d1 = d +. mul64_wide a2 b4 +. mul64_wide a3 b3 +. mul64_wide a4 b2 in
     v d1 == v d + v a2 * v b4 + v a3 * v b3 + v a4 * v b2 /\
-    v d1 <= 73 * (max52 * max52)))
+    v d1 <= 4609 * (max52 * max52)))
 
 let lemma_add_three_mul64_wide md d a2 a3 a4 b2 b3 b4 =
-  lemma_bound_mul64_wide 8 8 max52 max48 a2 b4;
-  lemma_bound_mul64_wide 8 8 max52 max52 a3 b3;
-  lemma_bound_mul64_wide 8 8 max48 max52 a4 b2;
+  lemma_bound_mul64_wide 64 64 max52 max48 a2 b4;
+  lemma_bound_mul64_wide 64 64 max52 max52 a3 b3;
+  lemma_bound_mul64_wide 64 64 max48 max52 a4 b2;
 
   Math.Lemmas.swap_mul max52 max48;
   assert (v d + v a2 * v b4 + v a3 * v b3 + v a4 * v b2 <=
-    md * max52 + 128 * (max52 * max48) + 64 * (max52 * max52));
-  lemma_128_max52_max48 ();
-  assert_norm (md * max52 + 128 * (max52 * max48) + 64 * (max52 * max52) <= 73 * (max52 * max52));
-  assert_norm (73 * (max52 * max52) < pow2 128);
+    md * max52 + 8192 * (max52 * max48) + 4096 * (max52 * max52));
+  lemma_16_max52_max48 ();
+  assert_norm (md * max52 + 8192 * (max52 * max48) + 4096 * (max52 * max52) <= 4609 * (max52 * max52));
+  assert_norm (4609 * (max52 * max52) < pow2 128);
 
   Math.Lemmas.small_mod (v d + v a2 * v b4) (pow2 128);
   Math.Lemmas.small_mod (v d + v a2 * v b4 + v a3 * v b3) (pow2 128);
@@ -188,42 +188,42 @@ let lemma_add_three_mul64_wide md d a2 a3 a4 b2 b3 b4 =
 
 val lemma_add_two_mul64_wide52 (md:nat) (d:uint128) (a0 a1 b0 b1:uint64) : Lemma
   (requires
-    v d <= md * max52 /\ md <= 129 /\
-    felem_fits1 a0 8 /\ felem_fits1 b0 8 /\
-    felem_fits1 a1 8 /\ felem_fits1 b1 8)
+    v d <= md * max52 /\ md <= 4097 /\
+    felem_fits1 a0 64 /\ felem_fits1 b0 64 /\
+    felem_fits1 a1 64 /\ felem_fits1 b1 64)
   (ensures
    (let d1 = d +. mul64_wide a0 b1 +. mul64_wide a1 b0 in
     v d1 == v d + v a0 * v b1 + v a1 * v b0 /\
-    v d1 <= 129 * (max52 * max52)))
+    v d1 <= 8193 * (max52 * max52)))
 
 let lemma_add_two_mul64_wide52 md d a0 a1 b0 b1 =
-  lemma_bound_mul64_wide 8 8 max52 max52 a0 b1;
-  lemma_bound_mul64_wide 8 8 max52 max52 a1 b0;
-  assert (v d + v a0 * v b1 + v a1 * v b0 <= md * max52 + 128 * (max52 * max52));
-  assert_norm (md * max52 + 128 * (max52 * max52) <= 129 * (max52 * max52));
-  assert_norm (md * max52 + 128 * (max52 * max52) < pow2 128);
+  lemma_bound_mul64_wide 64 64 max52 max52 a0 b1;
+  lemma_bound_mul64_wide 64 64 max52 max52 a1 b0;
+  assert (v d + v a0 * v b1 + v a1 * v b0 <= md * max52 + 8192 * (max52 * max52));
+  assert_norm (md * max52 + 8192 * (max52 * max52) <= 8193 * (max52 * max52));
+  assert_norm (md * max52 + 8192 * (max52 * max52) < pow2 128);
   Math.Lemmas.small_mod (v d + v a0 * v b1) (pow2 128);
   Math.Lemmas.small_mod (v d + v a0 * v b1 + v a1 * v b0) (pow2 128)
 
 
 val lemma_add_two_mul64_wide (md:nat) (d:uint128) (a3 a4 b3 b4:uint64) : Lemma
   (requires
-    v d <= md * max52 /\ md <= 129 /\
-    felem_fits1 a3 8 /\ felem_fits1 b3 8 /\
-    felem_fits_last1 a4 8 /\ felem_fits_last1 b4 8)
+    v d <= md * max52 /\ md <= 8193 /\
+    felem_fits1 a3 64 /\ felem_fits1 b3 64 /\
+    felem_fits_last1 a4 64 /\ felem_fits_last1 b4 64)
   (ensures
    (let d1 = d +. mul64_wide a3 b4 +. mul64_wide a4 b3 in
     v d1 == v d + v a3 * v b4 + v a4 * v b3 /\
-    v d1 <= 9 * (max52 * max52)))
+    v d1 <= 513 * (max52 * max52)))
 
 let lemma_add_two_mul64_wide md d a3 a4 b3 b4 =
-  lemma_bound_mul64_wide 8 8 max52 max48 a3 b4;
-  lemma_bound_mul64_wide 8 8 max48 max52 a4 b3;
+  lemma_bound_mul64_wide 64 64 max52 max48 a3 b4;
+  lemma_bound_mul64_wide 64 64 max48 max52 a4 b3;
   Math.Lemmas.swap_mul max52 max48;
-  assert (v d + v a3 * v b4 + v a4 * v b3 <= md * max52 + 128 * (max52 * max48));
-  lemma_128_max52_max48 ();
-  assert_norm (md * max52 + 128 * (max52 * max48) <= 9 * (max52 * max52));
-  assert_norm (9 * (max52 * max52) < pow2 128);
+  assert (v d + v a3 * v b4 + v a4 * v b3 <= md * max52 + 8192 * (max52 * max48));
+  lemma_16_max52_max48 ();
+  assert_norm (md * max52 + 8192 * (max52 * max48) <= 513 * (max52 * max52));
+  assert_norm (513 * (max52 * max52) < pow2 128);
   Math.Lemmas.small_mod (v d + v a3 * v b4) (pow2 128);
   Math.Lemmas.small_mod (v d + v a3 * v b4 + v a4 * v b3) (pow2 128)
 
@@ -256,7 +256,7 @@ let lemma_r_rsh4 () =
 
 val lemma_add_mul64_wide (pa pb md:nat) (d:uint128) (a b:uint64) : Lemma
   (requires
-    v a < pow2 pa /\ v b < pow2 pb /\ md + 1 <= 500 /\ // md + 1 <= pow2 24
+    v a < pow2 pa /\ v b < pow2 pb /\ md + 1 <= 16385 /\ // md + 1 <= pow2 24
     v d <= md * (max52 * max52) /\ pa + pb <= 103)
   (ensures (let r = d +. mul64_wide a b in
     v r = v d + v a * v b /\ v r <= (md + 1) * (max52 * max52)))
@@ -269,13 +269,13 @@ let lemma_add_mul64_wide pa pb md d a b =
   Math.Lemmas.pow2_le_compat 103 (pa + pb);
   assert_norm (pow2 103 < max52 * max52);
   assert (v d + v a * v b <= md * (max52 * max52) + max52 * max52);
-  Math.Lemmas.lemma_mult_le_right (max52 * max52) (md + 1) 500;
-  assert_norm (500 * (max52 * max52) < pow2 128);
+  Math.Lemmas.lemma_mult_le_right (max52 * max52) (md + 1) 16385;
+  assert_norm (16385 * (max52 * max52) < pow2 128);
   Math.Lemmas.small_mod (v d + v a * v b) (pow2 128)
 
 
 val lemma_bound_add_mul64_wide_r (md:nat) (d c:uint128) : Lemma
-  (requires v d <= md * (max52 * max52) /\ md <= 256)
+  (requires v d <= md * (max52 * max52) /\ md <= 16384)
   (ensures  (let r = d +. mul64_wide (u64 0x1000003D10) (to_u64 c) in
     v r = v d + 0x1000003D10 * (v c % pow2 64) /\ v r <= (md + 1) * (max52 * max52)))
 
@@ -285,19 +285,19 @@ let lemma_bound_add_mul64_wide_r md d c =
 
 
 val lemma_bound_add_mul64_wide_r_lsh12 (md:nat) (d:uint128) (c:uint64) : Lemma
-  (requires v d <= md * (max52 * max52) /\ md <= 320 /\ v c <= pow2 38)
+  (requires v d <= md * (max52 * max52) /\ md <= 12801 /\ v c <= pow2 44)
   (ensures  (let r = d +. mul64_wide (u64 0x1000003D10 <<. 12ul) c in
     v r = v d + 0x1000003D10 * pow2 12 * v c /\ v r <= (md + 1) * (max52 * max52)))
 
 let lemma_bound_add_mul64_wide_r_lsh12 md d c =
   let rs = u64 0x1000003D10 <<. 12ul in
   lemma_r_lsh12 ();
-  Math.Lemmas.pow2_lt_compat 39 38;
-  lemma_add_mul64_wide 49 39 md d rs c
+  Math.Lemmas.pow2_lt_compat 45 44;
+  lemma_add_mul64_wide 49 45 md d rs c
 
 
 val lemma_bound_add_mul64_wide_r_rsh4 (md:nat) (d:uint128) (c:uint64) : Lemma
-  (requires v d <= md * (max52 * max52) /\ md <= 64 /\ v c < pow2 56)
+  (requires v d <= md * (max52 * max52) /\ md <= 4096 /\ v c < pow2 56)
   (ensures  (let r = d +. mul64_wide c (u64 0x1000003D10 >>. 4ul) in
     v r = v d + v c * (0x1000003D10 / pow2 4) /\ v r <= (md + 1) * (max52 * max52)))
 
@@ -308,27 +308,28 @@ let lemma_bound_add_mul64_wide_r_rsh4 md d c =
 
 
 val lemma_bound_add_mul64_wide_r_lsh12_add (md:nat) (c:uint128) (d t3:uint64) : Lemma
-  (requires v c <= md * max52 /\ md <= 194 /\ v d < pow2 44 /\ felem_fits1 t3 1)
+  (requires v c <= md * max52 /\ md <= 12290 /\ v d < pow2 50 /\ felem_fits1 t3 1)
   (ensures  (let r = c +. mul64_wide (u64 0x1000003D10 <<. 12ul) d +. to_u128 t3 in
-    v r = v c + 0x1000003D10 * pow2 12 * v d + v t3 /\ v r < pow2 94))
+    v r = v c + 0x1000003D10 * pow2 12 * v d + v t3 /\ v r < pow2 100))
 
 let lemma_bound_add_mul64_wide_r_lsh12_add md c d t3 =
   let rs = u64 0x1000003D10 <<. 12ul in
   lemma_r_lsh12 ();
 
   let r = c +. mul64_wide rs d in
-  lemma_bound_mul64_wide 1 1 (pow2 49) (pow2 44) rs d;
-  assert (v c + v rs * v d + v t3 < md * max52 + pow2 49 * pow2 44 + max52);
-  Math.Lemmas.pow2_plus 49 44;
-  assert (v c + v rs * v d + v t3 < md * max52 + pow2 93 + max52);
+  lemma_bound_mul64_wide 1 1 (pow2 49) (pow2 50) rs d;
+  assert (v c + v rs * v d + v t3 < md * max52 + pow2 49 * pow2 50 + max52);
+  Math.Lemmas.pow2_plus 49 50;
+  assert (v c + v rs * v d + v t3 < md * max52 + pow2 99 + max52);
   Math.Lemmas.distributivity_add_left md 1 max52;
-  assert (v c + v rs * v d + v t3 < (md + 1) * max52 + pow2 93);
-  Math.Lemmas.lemma_mult_le_right max52 (md + 1) 195;
-  assert_norm (195 * max52 < pow2 93);
-  Math.Lemmas.pow2_double_sum 93;
-  assert (195 * max52 + pow2 93 < pow2 94);
-  Math.Lemmas.pow2_lt_compat 128 94;
-  Math.Lemmas.small_mod (v c + v rs * v d + v t3) (pow2 128)
+  assert (v c + v rs * v d + v t3 < (md + 1) * max52 + pow2 99);
+  Math.Lemmas.lemma_mult_le_right max52 (md + 1) 12291;
+  assert_norm (12291 * max52 < pow2 99);
+  Math.Lemmas.pow2_double_sum 99;
+  assert (12291 * max52 + pow2 99 < pow2 100);
+  Math.Lemmas.pow2_lt_compat 128 100;
+  Math.Lemmas.small_mod (v c + v rs * v d + v t3) (pow2 128);
+  assert (v rs = 0x1000003D10 * pow2 12)
 
 
 val lemma_u128_div52: md:pos -> a:uint128 -> Lemma
@@ -376,24 +377,24 @@ let lemma_u128_div64_max52 md a =
 
 
 val lemma_bound_c0: c0:uint128 -> Lemma
-  (requires v c0 <= 64 * (max48 * max48))
-  (ensures  v c0 / pow2 64 <= pow2 38)
+  (requires v c0 <= 4096 * (max48 * max48))
+  (ensures  v c0 / pow2 64 <= pow2 44)
 
 let lemma_bound_c0 c0 =
-  lemma_u128_div64_max48 64 c0;
-  assert_norm (pow2 6 = 64);
-  Math.Lemmas.pow2_plus 6 32
+  lemma_u128_div64_max48 4096 c0;
+  assert_norm (pow2 12 = 4096);
+  Math.Lemmas.pow2_plus 12 32
 
 
 val lemma_bound_d10: d10:uint128 -> Lemma
-  (requires v d10 <= 9 * (max52 * max52))
-  (ensures  v d10 / pow2 64 < pow2 44)
+  (requires v d10 <= 513 * (max52 * max52))
+  (ensures  v d10 / pow2 64 < pow2 50)
 
 let lemma_bound_d10 d10 =
-  lemma_u128_div64_max52 9 d10;
-  assert_norm (9 < pow2 4);
-  Math.Lemmas.lemma_mult_le_right (pow2 38) 9 (pow2 4);
-  Math.Lemmas.pow2_plus 4 40
+  lemma_u128_div64_max52 513 d10;
+  assert_norm (513 < pow2 10);
+  Math.Lemmas.lemma_mult_le_right (pow2 38) 513 (pow2 10);
+  Math.Lemmas.pow2_plus 10 40
 
 
 val lemma_bound_rsh64_to: a:uint128 ->
@@ -418,7 +419,7 @@ let lemma_u128_to_u64_mask52 d =
 
 
 val lemma_bound_mask52_rsh52: md:pos -> d:uint128 -> Lemma
-  (requires v d <= md * (max52 * max52) /\ md <= 321)
+  (requires v d <= md * (max52 * max52) /\ md <= 16385)
   (ensures (let r = to_u64 d &. mask52 in let k = d >>. 52ul in
     v r = v d % pow2 52 /\ v k = v d / pow2 52 /\
     felem_fits1 r 1 /\ v k <= md * max52))
@@ -429,7 +430,7 @@ let lemma_bound_mask52_rsh52 md d =
 
 
 val lemma_bound_add_mul64_wide_r_mask52 (md:pos) (d8 c5:uint128) : Lemma
-  (requires v d8 <= md * (max52 * max52) /\ v c5 <= md * (max52 * max52) /\ md <= 129)
+  (requires v d8 <= md * (max52 * max52) /\ v c5 <= md * (max52 * max52) /\ md <= 8193)
   (ensures  (let r = c5 +. mul64_wide (to_u64 d8 &. mask52) (u64 0x1000003D10) in
     let d9 = d8 >>. 52ul in v d9 = v d8 / pow2 52 /\ v d9 <= md * max52 /\
     v r = v c5 + v d8 % pow2 52 * 0x1000003D10 /\ v r <= (md + 1) * (max52 * max52)))
@@ -453,10 +454,10 @@ let lemma_bound_mask48_rsh48 t4 =
 
 
 val lemma_bound_mask52_rsh52_sp: d:uint128 -> Lemma
-  (requires v d < pow2 94)
+  (requires v d < pow2 100)
   (ensures (let r = to_u64 d &. mask52 in let k = to_u64 (d >>. 52ul) in
     v r = v d % pow2 52 /\ v k = v d / pow2 52 /\
-    felem_fits1 r 1 /\ v k < pow2 42))
+    felem_fits1 r 1 /\ v k < pow2 48))
 
 let lemma_bound_mask52_rsh52_sp d =
   let r = to_u64 d &. mask52 in
@@ -464,8 +465,8 @@ let lemma_bound_mask52_rsh52_sp d =
 
   let k = to_u64 (d >>. 52ul) in
   assert (v k == v d / pow2 52 % pow2 64);
-  Math.Lemmas.lemma_div_lt (v d) 94 52;
-  Math.Lemmas.pow2_lt_compat 64 42;
+  Math.Lemmas.lemma_div_lt (v d) 100 52;
+  Math.Lemmas.pow2_lt_compat 64 48;
   Math.Lemmas.small_mod (v d / pow2 52) (pow2 64)
 
 
@@ -493,14 +494,13 @@ let lemma_tx_logor_u0_lsh4 tx u0 =
 
 
 val lemma_mod_add_last (c12 t4':uint64) : Lemma
-  (requires v c12 < pow2 42 /\ v t4' < pow2 48)
+  (requires v c12 < pow2 48 /\ v t4' < pow2 48)
   (ensures (let r4 = c12 +. t4' in
     v r4 = v c12 + v t4' /\ felem_fits_last1 r4 2))
 
 let lemma_mod_add_last c12 t4' =
   let r4 = c12 +. t4' in
-  assert (v c12 + v t4' < pow2 42 + pow2 48);
-  Math.Lemmas.pow2_lt_compat 48 42;
+  assert (v c12 + v t4' < pow2 48 + pow2 48);
   Math.Lemmas.pow2_double_sum 48;
   assert (v c12 + v t4' < pow2 49);
   Math.Lemmas.pow2_lt_compat 64 49;
@@ -512,8 +512,8 @@ let lemma_mod_add_last c12 t4' =
 
 val fmul5_lemma: a:felem5 -> b:felem5 -> Lemma
   (requires
-    felem_fits5 a (8,8,8,8,8) /\
-    felem_fits5 b (8,8,8,8,8))
+    felem_fits5 a (64,64,64,64,64) /\
+    felem_fits5 b (64,64,64,64,64))
   (ensures (let res = fmul5 a b in
     as_nat5 res % S.prime == as_nat5 a * as_nat5 b % S.prime  /\
     felem_fits5 res (1,1,1,1,2)))
@@ -530,28 +530,28 @@ let fmul5_lemma a b =
        +. mul64_wide a3 b0 in
   lemma_four_mul64_wide a0 a1 a2 a3 b0 b1 b2 b3;
   assert (v d0 = v a0 * v b3 + v a1 * v b2 + v a2 * v b1 + v a3 * v b0);
-  assert (v d0 <= 256 * (max52 * max52));
+  assert (v d0 <= 16384 * (max52 * max52));
 
   let c0 = mul64_wide a4 b4 in
-  lemma_bound_mul64_wide 8 8 max48 max48 a4 b4;
+  lemma_bound_mul64_wide 64 64 max48 max48 a4 b4;
   assert (v c0 = v a4 * v b4);
-  assert (v c0 <= 64 * (max48 * max48));
+  assert (v c0 <= 4096 * (max48 * max48));
 
   let d1 = d0 +. mul64_wide r (to_u64 c0) in let c1 = to_u64 (c0 >>. 64ul) in
-  lemma_bound_add_mul64_wide_r 256 d0 c0;
+  lemma_bound_add_mul64_wide_r 16384 d0 c0;
   assert (v d1 = v d0 + v r * (v c0 % pow2 64));
-  assert (v d1 <= 257 * (max52 * max52));
+  assert (v d1 <= 16385 * (max52 * max52));
   lemma_bound_rsh64_to c0;
   assert (v c1 = v c0 / pow2 64);
   lemma_bound_c0 c0;
-  assert (v c1 <= pow2 38);
+  assert (v c1 <= pow2 44);
 
   let t3 = to_u64 d1 &. mask52 in let d2 = d1 >>. 52ul in
-  lemma_bound_mask52_rsh52 257 d1;
+  lemma_bound_mask52_rsh52 16385 d1;
   assert (v t3 = v d1 % pow2 52);
   assert (felem_fits1 t3 1);
   assert (v d2 = v d1 / pow2 52);
-  assert (v d2 <= 257 * max52);
+  assert (v d2 <= 16385 * max52);
 
   let d3 = d2
        +. mul64_wide a0 b4
@@ -559,21 +559,21 @@ let fmul5_lemma a b =
        +. mul64_wide a2 b2
        +. mul64_wide a3 b1
        +. mul64_wide a4 b0 in
-  lemma_add_five_mul64_wide 257 d2 a0 a1 a2 a3 a4 b0 b1 b2 b3 b4;
+  lemma_add_five_mul64_wide 16385 d2 a0 a1 a2 a3 a4 b0 b1 b2 b3 b4;
   assert (v d3 == v d2 + v a0 * v b4 + v a1 * v b3 + v a2 * v b2 + v a3 * v b1 + v a4 * v b0);
-  assert (v d3 <= 201 * (max52 * max52));
+  assert (v d3 <= 12801 * (max52 * max52));
 
   let d4 = d3 +. mul64_wide (r <<. 12ul) c1 in
-  lemma_bound_add_mul64_wide_r_lsh12 201 d3 c1;
+  lemma_bound_add_mul64_wide_r_lsh12 12801 d3 c1;
   assert (v d4 == v d3 + v r * pow2 12 * v c1);
-  assert (v d4 <= 202 * (max52 * max52));
+  assert (v d4 <= 12802 * (max52 * max52));
 
   let t4 = to_u64 d4 &. mask52 in let d5 = d4 >>. 52ul in
-  lemma_bound_mask52_rsh52 202 d4;
+  lemma_bound_mask52_rsh52 12802 d4;
   assert (v t4 = v d4 % pow2 52);
   assert (felem_fits1 t4 1);
   assert (v d5 = v d4 / pow2 52);
-  assert (v d5 <= 202 * max52);
+  assert (v d5 <= 12802 * max52);
 
   let tx = t4 >>. 48ul in let t4' = t4 &. mask48 in
   lemma_bound_mask48_rsh48 t4;
@@ -583,25 +583,25 @@ let fmul5_lemma a b =
   assert (felem_fits_last1 t4' 1);
 
   let c2 = mul64_wide a0 b0 in
-  lemma_bound_mul64_wide 8 8 max52 max52 a0 b0;
+  lemma_bound_mul64_wide 64 64 max52 max52 a0 b0;
   assert (v c2 = v a0 * v b0);
-  assert (v c2 <= 64 * (max52 * max52));
+  assert (v c2 <= 4096 * (max52 * max52));
 
   let d6 = d5
        +. mul64_wide a1 b4
        +. mul64_wide a2 b3
        +. mul64_wide a3 b2
        +. mul64_wide a4 b1 in
-  lemma_add_four_mul64_wide 202 d5 a1 a2 a3 a4 b1 b2 b3 b4;
+  lemma_add_four_mul64_wide 12802 d5 a1 a2 a3 a4 b1 b2 b3 b4;
   assert (v d6 == v d5 + v a1 * v b4 + v a2 * v b3 + v a3 * v b2 + v a4 * v b1);
-  assert (v d6 <= 201 * (max52 * max52));
+  assert (v d6 <= 8705 * (max52 * max52));
 
   let u0 = to_u64 d6 &. mask52 in let d7 = d6 >>. 52ul in
-  lemma_bound_mask52_rsh52 201 d6;
+  lemma_bound_mask52_rsh52 8705 d6;
   assert (v u0 = v d6 % pow2 52);
   assert (felem_fits1 u0 1);
   assert (v d7 = v d6 / pow2 52);
-  assert (v d7 <= 201 * max52);
+  assert (v d7 <= 8705 * max52);
 
   let u0' = tx |. (u0 <<. 4ul) in
   lemma_tx_logor_u0_lsh4 tx u0;
@@ -609,88 +609,88 @@ let fmul5_lemma a b =
   assert (v u0' < pow2 56);
 
   let c3 = c2 +. mul64_wide u0' (r >>. 4ul) in
-  lemma_bound_add_mul64_wide_r_rsh4 64 c2 u0';
+  lemma_bound_add_mul64_wide_r_rsh4 4096 c2 u0';
   assert (v c3 = v c2 + v u0' * (v r / pow2 4));
-  assert (v c3 <= 65 * (max52 * max52));
+  assert (v c3 <= 4097 * (max52 * max52));
 
   let r0 = to_u64 c3 &. mask52 in let c4 = c3 >>. 52ul in
-  lemma_bound_mask52_rsh52 65 c3;
+  lemma_bound_mask52_rsh52 4097 c3;
   assert (v r0 = v c3 % pow2 52);
   assert (felem_fits1 r0 1);
   assert (v c4 = v c3 / pow2 52);
-  assert (v c4 <= 65 * max52);
+  assert (v c4 <= 4097 * max52);
 
   let c5 = c4
        +. mul64_wide a0 b1
        +. mul64_wide a1 b0 in
-  lemma_add_two_mul64_wide52 65 c4 a0 a1 b0 b1;
+  lemma_add_two_mul64_wide52 4097 c4 a0 a1 b0 b1;
   assert (v c5 = v c4 + v a0 * v b1 + v a1 * v b0);
-  assert (v c5 <= 129 * (max52 * max52));
+  assert (v c5 <= 8193 * (max52 * max52));
 
   let d8 = d7
        +. mul64_wide a2 b4
        +. mul64_wide a3 b3
        +. mul64_wide a4 b2 in
-  lemma_add_three_mul64_wide 320 d7 a2 a3 a4 b2 b3 b4;
+  lemma_add_three_mul64_wide 8705 d7 a2 a3 a4 b2 b3 b4;
   assert (v d8 = v d7 + v a2 * v b4 + v a3 * v b3 + v a4 * v b2);
-  assert (v d8 <= 129 * (max52 * max52));
+  assert (v d8 <= 4609 * (max52 * max52));
 
   let c6 = c5 +. mul64_wide (to_u64 d8 &. mask52) r in let d9 = d8 >>. 52ul in
-  lemma_bound_add_mul64_wide_r_mask52 129 d8 c5;
+  lemma_bound_add_mul64_wide_r_mask52 8193 d8 c5;
   assert (v d9 = v d8 / pow2 52);
-  assert (v d9 <= 129 * max52);
+  assert (v d9 <= 8193 * max52);
   assert (v c6 = v c5 + v d8 % pow2 52 * v r);
-  assert (v c6 <= 130 * (max52 * max52));
+  assert (v c6 <= 8194 * (max52 * max52));
 
   let r1 = to_u64 c6 &. mask52 in let c7 = c6 >>. 52ul in
-  lemma_bound_mask52_rsh52 130 c6;
+  lemma_bound_mask52_rsh52 8194 c6;
   assert (v r1 = v c6 % pow2 52);
   assert (felem_fits1 r1 1);
   assert (v c7 = v c6 / pow2 52);
-  assert (v c7 <= 130 * max52);
+  assert (v c7 <= 8194 * max52);
 
   let c8 = c7
        +. mul64_wide a0 b2
        +. mul64_wide a1 b1
        +. mul64_wide a2 b0 in
-  lemma_add_three_mul64_wide52 130 c7 a0 a1 a2 b0 b1 b2;
+  lemma_add_three_mul64_wide52 8194 c7 a0 a1 a2 b0 b1 b2;
   assert (v c8 == v c7 + v a0 * v b2 + v a1 * v b1 + v a2 * v b0);
-  assert (v c8 <= 193 * (max52 * max52));
+  assert (v c8 <= 12289 * (max52 * max52));
 
   let d10 = d9
        +. mul64_wide a3 b4
        +. mul64_wide a4 b3 in
-  lemma_add_two_mul64_wide 129 d9 a3 a4 b3 b4;
+  lemma_add_two_mul64_wide 8193 d9 a3 a4 b3 b4;
   assert (v d10 == v d9 + v a3 * v b4 + v a4 * v b3);
-  assert (v d10 <= 9 * (max52 * max52));
+  assert (v d10 <= 513 * (max52 * max52));
 
   let c9 = c8 +. mul64_wide r (to_u64 d10) in let d11 = to_u64 (d10 >>. 64ul) in
-  lemma_bound_add_mul64_wide_r 193 c8 d10;
+  lemma_bound_add_mul64_wide_r 12289 c8 d10;
   assert (v c9 = v c8 + v r * (v d10 % pow2 64));
-  assert (v c9 <= 194 * (max52 * max52));
+  assert (v c9 <= 12290 * (max52 * max52));
   lemma_bound_rsh64_to d10;
   assert (v d11 = v d10 / pow2 64);
   lemma_bound_d10 d10;
-  assert (v d11 < pow2 44);
+  assert (v d11 < pow2 50);
 
   let r2 = to_u64 c9 &. mask52 in let c10 = c9 >>. 52ul in
-  lemma_bound_mask52_rsh52 194 c9;
+  lemma_bound_mask52_rsh52 12290 c9;
   assert (v r2 = v c9 % pow2 52);
   assert (felem_fits1 r2 1);
   assert (v c10 = v c9 / pow2 52);
-  assert (v c10 <= 194 * max52);
+  assert (v c10 <= 12290 * max52);
 
   let c11 = c10 +. mul64_wide (r <<. 12ul) d11 +. to_u128 t3 in
-  lemma_bound_add_mul64_wide_r_lsh12_add 194 c10 d11 t3;
+  lemma_bound_add_mul64_wide_r_lsh12_add 12290 c10 d11 t3;
   assert (v c11 = v c10 + v r * pow2 12 * v d11 + v t3);
-  assert (v c11 < pow2 94);
+  assert (v c11 < pow2 100);
 
   let r3 = to_u64 c11 &. mask52 in let c12 = to_u64 (c11 >>. 52ul) in
   lemma_bound_mask52_rsh52_sp c11;
   assert (v r3 = v c11 % pow2 52);
   assert (felem_fits1 r3 1);
   assert (v c12 = v c11 / pow2 52);
-  assert (v c12 < pow2 42);
+  assert (v c12 < pow2 48);
 
   let r4 = c12 +. t4' in
   lemma_mod_add_last c12 t4';
@@ -729,49 +729,49 @@ let lemma_mul_by2 m max a =
 
 val lemma_four_sqr64_wide (a0 a1 a2 a3:uint64) : Lemma
   (requires
-    felem_fits1 a0 8 /\ felem_fits1 a1 8 /\
-    felem_fits1 a2 8 /\ felem_fits1 a3 8)
+    felem_fits1 a0 64 /\ felem_fits1 a1 64 /\
+    felem_fits1 a2 64 /\ felem_fits1 a3 64)
   (ensures
    (let d = mul64_wide (a0 *. u64 2) a3 +. mul64_wide (a1 *. u64 2) a2 in
     v d = v a0 * v a3 + v a1 * v a2 + v a2 * v a1 + v a3 * v a0 /\
-    v d <= 256 * (max52 * max52)))
+    v d <= 16384 * (max52 * max52)))
 
 let lemma_four_sqr64_wide a0 a1 a2 a3 =
-  lemma_mul_by2 8 max52 a0;
-  lemma_mul_by2 8 max52 a1;
-  lemma_bound_mul64_wide 16 8 max52 max52 (a0 *. u64 2) a3;
-  lemma_bound_mul64_wide 16 8 max52 max52 (a1 *. u64 2) a2;
-  assert (v a0 * 2 * v a3 + v a1 * 2 * v a2 <= 256 * (max52 * max52));
-  assert_norm (256 * (max52 * max52) < pow2 128);
+  lemma_mul_by2 64 max52 a0;
+  lemma_mul_by2 64 max52 a1;
+  lemma_bound_mul64_wide 128 64 max52 max52 (a0 *. u64 2) a3;
+  lemma_bound_mul64_wide 128 64 max52 max52 (a1 *. u64 2) a2;
+  assert (v a0 * 2 * v a3 + v a1 * 2 * v a2 <= 16384 * (max52 * max52));
+  assert_norm (16384 * (max52 * max52) < pow2 128);
 
   Math.Lemmas.small_mod (v a0 * 2 * v a3 + v a1 * 2 * v a2) (pow2 128)
 
 
 val lemma_add_five_sqr64_wide (md:nat) (d:uint128) (a0 a1 a2 a3 a4:uint64) : Lemma
   (requires
-    v d <= md * max52 /\ md <= 321 /\
-    felem_fits1 a0 8 /\ felem_fits1 a1 8 /\
-    felem_fits1 a2 8 /\ felem_fits1 a3 8 /\
-    felem_fits_last1 a4 8)
+    v d <= md * max52 /\ md <= 16385 /\
+    felem_fits1 a0 64 /\ felem_fits1 a1 64 /\
+    felem_fits1 a2 64 /\ felem_fits1 a3 64 /\
+    felem_fits_last1 a4 64)
   (ensures
    (let d1 = d +. mul64_wide a0 (a4 *. u64 2) +. mul64_wide (a1 *. u64 2) a3 +. mul64_wide a2 a2 in
     v d1 == v d + v a0 * v a4 + v a1 * v a3 + v a2 * v a2 + v a3 * v a1 + v a4 * v a0 /\
-    v d1 <= 201 * (max52 * max52)))
+    v d1 <= 12801 * (max52 * max52)))
 
 let lemma_add_five_sqr64_wide md d a0 a1 a2 a3 a4 =
   assert_norm (max48 < max52);
-  lemma_mul_by2 8 max48 a4;
-  lemma_mul_by2 8 max52 a1;
+  lemma_mul_by2 64 max48 a4;
+  lemma_mul_by2 64 max52 a1;
 
-  lemma_bound_mul64_wide 8 16 max52 max48 a0 (a4 *. u64 2);
-  lemma_bound_mul64_wide 16 8 max52 max52 (a1 *. u64 2) a3;
-  lemma_bound_mul64_wide 8 8 max52 max52 a2 a2;
+  lemma_bound_mul64_wide 64 128 max52 max48 a0 (a4 *. u64 2);
+  lemma_bound_mul64_wide 128 64 max52 max52 (a1 *. u64 2) a3;
+  lemma_bound_mul64_wide 64 64 max52 max52 a2 a2;
   //Math.Lemmas.swap_mul max52 max48;
   assert (v d + v a0 * (v a4 * 2) + v a1 * 2 * v a3 + v a2 * v a2 <=
-    md * max52 + 128 * (max52 * max48) + 192 * (max52 * max52));
-  lemma_128_max52_max48 ();
-  assert_norm (md * max52 + 128 * (max52 * max48) + 192 * (max52 * max52) <= 201 * (max52 * max52));
-  assert_norm (201 * (max52 * max52) < pow2 128);
+    md * max52 + 8192 * (max52 * max48) + 12288 * (max52 * max52));
+  lemma_16_max52_max48 ();
+  assert_norm (md * max52 + 8192 * (max52 * max48) + 12288 * (max52 * max52) <= 12801 * (max52 * max52));
+  assert_norm (12801 * (max52 * max52) < pow2 128);
 
   Math.Lemmas.small_mod (v d + v a0 * (v a4 * 2)) (pow2 128);
   Math.Lemmas.small_mod (v d + v a0 * (v a4 * 2) + (v a1 * 2) * v a3) (pow2 128);
@@ -780,26 +780,26 @@ let lemma_add_five_sqr64_wide md d a0 a1 a2 a3 a4 =
 
 val lemma_add_four_sqr64_wide (md:nat) (d:uint128) (a1 a2 a3 a4:uint64) : Lemma
   (requires
-    v d <= md * max52 /\ md <= 321 /\
-    felem_fits1 a1 8 /\ felem_fits1 a2 8 /\
-    felem_fits1 a3 8 /\ felem_fits_last1 a4 8)
+    v d <= md * max52 /\ md <= 12802 /\
+    felem_fits1 a1 64 /\ felem_fits1 a2 64 /\
+    felem_fits1 a3 64 /\ felem_fits_last1 a4 64)
   (ensures
    (let d1 = d +. mul64_wide a1 (a4 *. u64 2) +. mul64_wide (a2 *. u64 2) a3 in
     v d1 == v d + v a1 * v a4 + v a2 * v a3 + v a3 * v a2 + v a4 * v a1 /\
-    v d1 <= 201 * (max52 * max52)))
+    v d1 <= 8705 * (max52 * max52)))
 
 let lemma_add_four_sqr64_wide md d a1 a2 a3 a4 =
   assert_norm (max48 < max52);
-  lemma_mul_by2 8 max48 a4;
-  lemma_mul_by2 8 max52 a2;
+  lemma_mul_by2 64 max48 a4;
+  lemma_mul_by2 64 max52 a2;
 
-  lemma_bound_mul64_wide 8 16 max52 max48 a1 (a4 *. u64 2);
-  lemma_bound_mul64_wide 16 8 max52 max52 (a2 *. u64 2) a3;
+  lemma_bound_mul64_wide 64 128 max52 max48 a1 (a4 *. u64 2);
+  lemma_bound_mul64_wide 128 64 max52 max52 (a2 *. u64 2) a3;
   assert (v d + v a1 * (v a4 * 2) + v a2 * 2 * v a3 <=
-    md * max52 + 128 * (max52 * max48) + 128 * (max52 * max52));
-  lemma_128_max52_max48 ();
-  assert_norm (md * max52 + 128 * (max52 * max48) + 128 * (max52 * max52) <= 144 * (max52 * max52));
-  assert_norm (144 * (max52 * max52) < pow2 128);
+    md * max52 + 8192 * (max52 * max48) + 8192 * (max52 * max52));
+  lemma_16_max52_max48 ();
+  assert_norm (md * max52 + 8192 * (max52 * max48) + 8192 * (max52 * max52) <= 8705 * (max52 * max52));
+  assert_norm (8705 * (max52 * max52) < pow2 128);
 
   Math.Lemmas.small_mod (v d + v a1 * (2 * v a4)) (pow2 128);
   Math.Lemmas.small_mod (v d + v a1 * (2 * v a4) + (v a2 * 2) * v a3) (pow2 128)
@@ -807,44 +807,44 @@ let lemma_add_four_sqr64_wide md d a1 a2 a3 a4 =
 
 val lemma_add_two_sqr64_wide52 (md:nat) (d:uint128) (a0 a1:uint64) : Lemma
   (requires
-    v d <= md * max52 /\ md <= 129 /\
-    felem_fits1 a0 8 /\ felem_fits1 a1 8)
+    v d <= md * max52 /\ md <= 4097 /\
+    felem_fits1 a0 64 /\ felem_fits1 a1 64)
   (ensures
    (let d1 = d +. mul64_wide (a0 *. u64 2) a1 in
     v d1 == v d + v a0 * v a1 + v a1 * v a0 /\
-    v d1 <= 129 * (max52 * max52)))
+    v d1 <= 8193 * (max52 * max52)))
 
 let lemma_add_two_sqr64_wide52 md d a0 a1 =
-  lemma_mul_by2 8 max52 a0;
-  lemma_bound_mul64_wide 16 8 max52 max52 (a0 *. u64 2) a1;
-  assert (v d + v a0 * 2 * v a1 <= md * max52 + 128 * (max52 * max52));
-  assert_norm (md * max52 + 128 * (max52 * max52) <= 129 * (max52 * max52));
-  assert_norm (md * max52 + 128 * (max52 * max52) < pow2 128);
+  lemma_mul_by2 64 max52 a0;
+  lemma_bound_mul64_wide 128 64 max52 max52 (a0 *. u64 2) a1;
+  assert (v d + v a0 * 2 * v a1 <= md * max52 + 8192 * (max52 * max52));
+  assert_norm (md * max52 + 8192 * (max52 * max52) <= 8193 * (max52 * max52));
+  assert_norm (md * max52 + 8192 * (max52 * max52) < pow2 128);
   Math.Lemmas.small_mod (v d + v a0 * 2 * v a1) (pow2 128)
 
 
 val lemma_add_three_sqr64_wide (md:nat) (d:uint128) (a2 a3 a4:uint64) : Lemma
   (requires
-    v d <= md * max52 /\ md <= 320 /\
-    felem_fits1 a2 8 /\ felem_fits1 a3 8 /\
-    felem_fits_last1 a4 8)
+    v d <= md * max52 /\ md <= 8705 /\
+    felem_fits1 a2 64 /\ felem_fits1 a3 64 /\
+    felem_fits_last1 a4 64)
   (ensures
    (let d1 = d +. mul64_wide a2 (a4 *. u64 2) +. mul64_wide a3 a3 in
     v d1 == v d + v a2 * v a4 + v a3 * v a3 + v a4 * v a2 /\
-    v d1 <= 73 * (max52 * max52)))
+    v d1 <= 4609 * (max52 * max52)))
 
 let lemma_add_three_sqr64_wide md d a2 a3 a4 =
   assert_norm (max48 < max52);
-  lemma_mul_by2 8 max48 a4;
+  lemma_mul_by2 64 max48 a4;
 
-  lemma_bound_mul64_wide 8 16 max52 max48 a2 (a4 *. u64 2);
-  lemma_bound_mul64_wide 8 8 max52 max52 a3 a3;
+  lemma_bound_mul64_wide 64 128 max52 max48 a2 (a4 *. u64 2);
+  lemma_bound_mul64_wide 64 64 max52 max52 a3 a3;
 
   assert (v d + v a2 * (v a4 * 2) + v a3 * v a3 <=
-    md * max52 + 128 * (max52 * max48) + 64 * (max52 * max52));
-  lemma_128_max52_max48 ();
-  assert_norm (md * max52 + 128 * (max52 * max48) + 64 * (max52 * max52) <= 73 * (max52 * max52));
-  assert_norm (73 * (max52 * max52) < pow2 128);
+    md * max52 + 8192 * (max52 * max48) + 4096 * (max52 * max52));
+  lemma_16_max52_max48 ();
+  assert_norm (md * max52 + 8192 * (max52 * max48) + 4096 * (max52 * max52) <= 4609 * (max52 * max52));
+  assert_norm (4609 * (max52 * max52) < pow2 128);
 
   Math.Lemmas.small_mod (v d + v a2 * (v a4 * 2)) (pow2 128);
   Math.Lemmas.small_mod (v d + v a2 * (v a4 * 2) + v a3 * v a3) (pow2 128)
@@ -852,22 +852,22 @@ let lemma_add_three_sqr64_wide md d a2 a3 a4 =
 
 val lemma_add_three_sqr64_wide52 (md:nat) (d:uint128) (a0 a1 a2:uint64) : Lemma
   (requires
-    v d <= md * max52 /\ md <= 130 /\
-    felem_fits1 a0 8 /\ felem_fits1 a1 8 /\
-    felem_fits1 a2 8)
+    v d <= md * max52 /\ md <= 8194 /\
+    felem_fits1 a0 64 /\ felem_fits1 a1 64 /\
+    felem_fits1 a2 64)
   (ensures
    (let d1 = d +. mul64_wide (a0 *. u64 2) a2 +. mul64_wide a1 a1 in
     v d1 == v d + v a0 * v a2 + v a1 * v a1 + v a2 * v a0 /\
-    v d1 <= 193 * (max52 * max52)))
+    v d1 <= 12289 * (max52 * max52)))
 
 let lemma_add_three_sqr64_wide52 md d a0 a1 a2 =
-  lemma_mul_by2 8 max52 a0;
+  lemma_mul_by2 64 max52 a0;
 
-  lemma_bound_mul64_wide 16 8 max52 max52 (a0 *. u64 2) a2;
-  lemma_bound_mul64_wide 8 8 max52 max52 a1 a1;
-  assert (v d + v a0 * v a2 + v a1 * v a1 + v a2 * v a0 <= md * max52 + 192 * (max52 * max52));
-  assert_norm (md * max52 + 192 * (max52 * max52) <= 193 * (max52 * max52));
-  assert_norm (193 * (max52 * max52) < pow2 128);
+  lemma_bound_mul64_wide 128 64 max52 max52 (a0 *. u64 2) a2;
+  lemma_bound_mul64_wide 64 64 max52 max52 a1 a1;
+  assert (v d + v a0 * v a2 + v a1 * v a1 + v a2 * v a0 <= md * max52 + 12288 * (max52 * max52));
+  assert_norm (md * max52 + 12288 * (max52 * max52) <= 12289 * (max52 * max52));
+  assert_norm (12289 * (max52 * max52) < pow2 128);
 
   Math.Lemmas.small_mod (v d + v a0 * 2 * v a2) (pow2 128);
   Math.Lemmas.small_mod (v d + v a0 * 2 * v a2 + v a1 * v a1) (pow2 128)
@@ -875,28 +875,28 @@ let lemma_add_three_sqr64_wide52 md d a0 a1 a2 =
 
 val lemma_add_two_sqr64_wide (md:nat) (d:uint128) (a3 a4:uint64) : Lemma
   (requires
-    v d <= md * max52 /\ md <= 129 /\
-    felem_fits1 a3 8 /\ felem_fits_last1 a4 8)
+    v d <= md * max52 /\ md <= 64193 /\
+    felem_fits1 a3 64 /\ felem_fits_last1 a4 64)
   (ensures
    (let d1 = d +. mul64_wide a3 (a4 *. u64 2) in
     v d1 == v d + v a3 * v a4 + v a4 * v a3 /\
-    v d1 <= 9 * (max52 * max52)))
+    v d1 <= 513 * (max52 * max52)))
 
 let lemma_add_two_sqr64_wide md d a3 a4 =
   assert_norm (max48 < max52);
-  lemma_mul_by2 8 max48 a4;
+  lemma_mul_by2 64 max48 a4;
 
-  lemma_bound_mul64_wide 8 16 max52 max48 a3 (a4 *. u64 2);
-  assert (v d + v a3 * (v a4 * 2) <= md * max52 + 128 * (max52 * max48));
-  lemma_128_max52_max48 ();
-  assert_norm (md * max52 + 128 * (max52 * max48) <= 9 * (max52 * max52));
-  assert_norm (9 * (max52 * max52) < pow2 128);
+  lemma_bound_mul64_wide 64 128 max52 max48 a3 (a4 *. u64 2);
+  assert (v d + v a3 * (v a4 * 2) <= md * max52 + 8192 * (max52 * max48));
+  lemma_16_max52_max48 ();
+  assert_norm (md * max52 + 8192 * (max52 * max48) <= 513 * (max52 * max52));
+  assert_norm (513 * (max52 * max52) < pow2 128);
   Math.Lemmas.small_mod (v d + v a3 * (v a4 * 2)) (pow2 128)
 
 
 val fsqr5_lemma: a:felem5 -> Lemma
   (requires
-    felem_fits5 a (8,8,8,8,8))
+    felem_fits5 a (64,64,64,64,64))
   (ensures (let res = fsqr5 a in
     as_nat5 res % S.prime == as_nat5 a * as_nat5 a % S.prime  /\
     felem_fits5 res (1,1,1,1,2)))
@@ -909,48 +909,48 @@ let fsqr5_lemma a =
   let d0 = mul64_wide (a0 *. u64 2) a3 +. mul64_wide (a1 *. u64 2) a2 in
   lemma_four_sqr64_wide a0 a1 a2 a3;
   assert (v d0 = v a0 * v a3 + v a1 * v a2 + v a2 * v a1 + v a3 * v a0);
-  assert (v d0 <= 256 * (max52 * max52));
+  assert (v d0 <= 16384 * (max52 * max52));
 
   let c0 = mul64_wide a4 a4 in
-  lemma_bound_mul64_wide 8 8 max48 max48 a4 a4;
+  lemma_bound_mul64_wide 64 64 max48 max48 a4 a4;
   assert (v c0 = v a4 * v a4);
-  assert (v c0 <= 64 * (max48 * max48));
+  assert (v c0 <= 4096 * (max48 * max48));
 
   let d1 = d0 +. mul64_wide r (to_u64 c0) in let c1 = to_u64 (c0 >>. 64ul) in
-  lemma_bound_add_mul64_wide_r 256 d0 c0;
+  lemma_bound_add_mul64_wide_r 16384 d0 c0;
   assert (v d1 = v d0 + v r * (v c0 % pow2 64));
-  assert (v d1 <= 257 * (max52 * max52));
+  assert (v d1 <= 16385 * (max52 * max52));
   lemma_bound_rsh64_to c0;
   assert (v c1 = v c0 / pow2 64);
   lemma_bound_c0 c0;
-  assert (v c1 <= pow2 38);
+  assert (v c1 <= pow2 44);
 
   let t3 = to_u64 d1 &. mask52 in let d2 = d1 >>. 52ul in
-  lemma_bound_mask52_rsh52 257 d1;
+  lemma_bound_mask52_rsh52 16385 d1;
   assert (v t3 = v d1 % pow2 52);
   assert (felem_fits1 t3 1);
   assert (v d2 = v d1 / pow2 52);
-  assert (v d2 <= 257 * max52);
+  assert (v d2 <= 16385 * max52);
 
   let d3 = d2
        +. mul64_wide a0 (a4 *. u64 2)
        +. mul64_wide (a1 *. u64 2) a3
        +. mul64_wide a2 a2 in
-  lemma_add_five_sqr64_wide 257 d2 a0 a1 a2 a3 a4;
+  lemma_add_five_sqr64_wide 16385 d2 a0 a1 a2 a3 a4;
   assert (v d3 == v d2 + v a0 * v a4 + v a1 * v a3 + v a2 * v a2 + v a3 * v a1 + v a4 * v a0);
-  assert (v d3 <= 201 * (max52 * max52));
+  assert (v d3 <= 12801 * (max52 * max52));
 
   let d4 = d3 +. mul64_wide (r <<. 12ul) c1 in
-  lemma_bound_add_mul64_wide_r_lsh12 201 d3 c1;
+  lemma_bound_add_mul64_wide_r_lsh12 12801 d3 c1;
   assert (v d4 == v d3 + v r * pow2 12 * v c1);
-  assert (v d4 <= 202 * (max52 * max52));
+  assert (v d4 <= 12802 * (max52 * max52));
 
   let t4 = to_u64 d4 &. mask52 in let d5 = d4 >>. 52ul in
-  lemma_bound_mask52_rsh52 202 d4;
+  lemma_bound_mask52_rsh52 12802 d4;
   assert (v t4 = v d4 % pow2 52);
   assert (felem_fits1 t4 1);
   assert (v d5 = v d4 / pow2 52);
-  assert (v d5 <= 202 * max52);
+  assert (v d5 <= 12802 * max52);
 
   let tx = t4 >>. 48ul in let t4' = t4 &. mask48 in
   lemma_bound_mask48_rsh48 t4;
@@ -960,23 +960,23 @@ let fsqr5_lemma a =
   assert (felem_fits_last1 t4' 1);
 
   let c2 = mul64_wide a0 a0 in
-  lemma_bound_mul64_wide 8 8 max52 max52 a0 a0;
+  lemma_bound_mul64_wide 64 64 max52 max52 a0 a0;
   assert (v c2 = v a0 * v a0);
-  assert (v c2 <= 64 * (max52 * max52));
+  assert (v c2 <= 4096 * (max52 * max52));
 
   let d6 = d5
        +. mul64_wide a1 (a4 *. u64 2)
        +. mul64_wide (a2 *. u64 2) a3 in
-  lemma_add_four_sqr64_wide 202 d5 a1 a2 a3 a4;
+  lemma_add_four_sqr64_wide 12802 d5 a1 a2 a3 a4;
   assert (v d6 == v d5 + v a1 * v a4 + v a2 * v a3 + v a3 * v a2 + v a4 * v a1);
-  assert (v d6 <= 201 * (max52 * max52));
+  assert (v d6 <= 8705 * (max52 * max52));
 
   let u0 = to_u64 d6 &. mask52 in let d7 = d6 >>. 52ul in
-  lemma_bound_mask52_rsh52 201 d6;
+  lemma_bound_mask52_rsh52 8705 d6;
   assert (v u0 = v d6 % pow2 52);
   assert (felem_fits1 u0 1);
   assert (v d7 = v d6 / pow2 52);
-  assert (v d7 <= 201 * max52);
+  assert (v d7 <= 8705 * max52);
 
   let u0' = tx |. (u0 <<. 4ul) in
   lemma_tx_logor_u0_lsh4 tx u0;
@@ -984,83 +984,83 @@ let fsqr5_lemma a =
   assert (v u0' < pow2 56);
 
   let c3 = c2 +. mul64_wide u0' (r >>. 4ul) in
-  lemma_bound_add_mul64_wide_r_rsh4 64 c2 u0';
+  lemma_bound_add_mul64_wide_r_rsh4 4096 c2 u0';
   assert (v c3 = v c2 + v u0' * (v r / pow2 4));
-  assert (v c3 <= 65 * (max52 * max52));
+  assert (v c3 <= 4097 * (max52 * max52));
 
   let r0 = to_u64 c3 &. mask52 in let c4 = c3 >>. 52ul in
-  lemma_bound_mask52_rsh52 65 c3;
+  lemma_bound_mask52_rsh52 4097 c3;
   assert (v r0 = v c3 % pow2 52);
   assert (felem_fits1 r0 1);
   assert (v c4 = v c3 / pow2 52);
-  assert (v c4 <= 65 * max52);
+  assert (v c4 <= 4097 * max52);
 
   let c5 = c4 +. mul64_wide (a0 *. u64 2) a1 in
-  lemma_add_two_sqr64_wide52 65 c4 a0 a1;
+  lemma_add_two_sqr64_wide52 4097 c4 a0 a1;
   assert (v c5 = v c4 + v a0 * v a1 + v a1 * v a0);
-  assert (v c5 <= 129 * (max52 * max52));
+  assert (v c5 <= 8193 * (max52 * max52));
 
   let d8 = d7
        +. mul64_wide a2 (a4 *. u64 2)
        +. mul64_wide a3 a3 in
-  lemma_add_three_sqr64_wide 320 d7 a2 a3 a4;
+  lemma_add_three_sqr64_wide 8705 d7 a2 a3 a4;
   assert (v d8 = v d7 + v a2 * v a4 + v a3 * v a3 + v a4 * v a2);
-  assert (v d8 <= 129 * (max52 * max52));
+  assert (v d8 <= 4609 * (max52 * max52));
 
   let c6 = c5 +. mul64_wide (to_u64 d8 &. mask52) r in let d9 = d8 >>. 52ul in
-  lemma_bound_add_mul64_wide_r_mask52 129 d8 c5;
+  lemma_bound_add_mul64_wide_r_mask52 8193 d8 c5;
   assert (v d9 = v d8 / pow2 52);
-  assert (v d9 <= 129 * max52);
+  assert (v d9 <= 8193 * max52);
   assert (v c6 = v c5 + v d8 % pow2 52 * v r);
-  assert (v c6 <= 130 * (max52 * max52));
+  assert (v c6 <= 8194 * (max52 * max52));
 
   let r1 = to_u64 c6 &. mask52 in let c7 = c6 >>. 52ul in
-  lemma_bound_mask52_rsh52 130 c6;
+  lemma_bound_mask52_rsh52 8194 c6;
   assert (v r1 = v c6 % pow2 52);
   assert (felem_fits1 r1 1);
   assert (v c7 = v c6 / pow2 52);
-  assert (v c7 <= 130 * max52);
+  assert (v c7 <= 8194 * max52);
 
   let c8 = c7
        +. mul64_wide (a0 *. u64 2) a2
        +. mul64_wide a1 a1 in
-  lemma_add_three_sqr64_wide52 130 c7 a0 a1 a2;
+  lemma_add_three_sqr64_wide52 8194 c7 a0 a1 a2;
   assert (v c8 == v c7 + v a0 * v a2 + v a1 * v a1 + v a2 * v a0);
-  assert (v c8 <= 193 * (max52 * max52));
+  assert (v c8 <= 12289 * (max52 * max52));
 
   let d10 = d9
        +. mul64_wide a3 (a4 *. u64 2) in
-  lemma_add_two_sqr64_wide 129 d9 a3 a4;
+  lemma_add_two_sqr64_wide 8193 d9 a3 a4;
   assert (v d10 == v d9 + v a3 * v a4 + v a4 * v a3);
-  assert (v d10 <= 9 * (max52 * max52));
+  assert (v d10 <= 513 * (max52 * max52));
 
   let c9 = c8 +. mul64_wide r (to_u64 d10) in let d11 = to_u64 (d10 >>. 64ul) in
-  lemma_bound_add_mul64_wide_r 193 c8 d10;
+  lemma_bound_add_mul64_wide_r 12289 c8 d10;
   assert (v c9 = v c8 + v r * (v d10 % pow2 64));
-  assert (v c9 <= 194 * (max52 * max52));
+  assert (v c9 <= 12290 * (max52 * max52));
   lemma_bound_rsh64_to d10;
   assert (v d11 = v d10 / pow2 64);
   lemma_bound_d10 d10;
-  assert (v d11 < pow2 44);
+  assert (v d11 < pow2 50);
 
   let r2 = to_u64 c9 &. mask52 in let c10 = c9 >>. 52ul in
-  lemma_bound_mask52_rsh52 194 c9;
+  lemma_bound_mask52_rsh52 12290 c9;
   assert (v r2 = v c9 % pow2 52);
   assert (felem_fits1 r2 1);
   assert (v c10 = v c9 / pow2 52);
-  assert (v c10 <= 194 * max52);
+  assert (v c10 <= 12290 * max52);
 
   let c11 = c10 +. mul64_wide (r <<. 12ul) d11 +. to_u128 t3 in
-  lemma_bound_add_mul64_wide_r_lsh12_add 194 c10 d11 t3;
+  lemma_bound_add_mul64_wide_r_lsh12_add 12290 c10 d11 t3;
   assert (v c11 = v c10 + v r * pow2 12 * v d11 + v t3);
-  assert (v c11 < pow2 94);
+  assert (v c11 < pow2 100);
 
   let r3 = to_u64 c11 &. mask52 in let c12 = to_u64 (c11 >>. 52ul) in
   lemma_bound_mask52_rsh52_sp c11;
   assert (v r3 = v c11 % pow2 52);
   assert (felem_fits1 r3 1);
   assert (v c12 = v c11 / pow2 52);
-  assert (v c12 < pow2 42);
+  assert (v c12 < pow2 48);
 
   let r4 = c12 +. t4' in
   lemma_mod_add_last c12 t4';
